progress on the invntt proof

proof/correctness/avx2/NTT_AVX_j.ec
@@ -636,46 +636,7 @@ move: Ha; rewrite -{1}iotaredE /R2C /= => |> *.
 move: Hb; rewrite -{1}iotaredE /R2C /= => |> *.
 by rewrite -!iotaredE /= /#.
 qed.
-(*
-hoare __shuffle8_h n _a _b:
- Jkem_avx2.M.__shuffle8:
-   I16u16_sb n a _a /\ I16u16_sb n b _b
-   ==> I16u16_sb n res.`1 (shuffle8 _a _b).`1
-       /\ I16u16_sb n res.`2 (shuffle8 _a _b).`2.
-proof.
-proc; simplify.
-wp; skip => |> &m Ha Hb.
-rewrite /VPERM2I128 /=.
-rewrite ifF.
- by rewrite /W8.of_int /= /int2bs /mkseq -iotaredE /=.
-rewrite ifF.
- by rewrite /W8.of_int /= /int2bs /mkseq -iotaredE /=.
-rewrite ifF.
- by rewrite /W8.of_int /= /int2bs /mkseq -iotaredE /=.
-rewrite ifT.
- by rewrite /W8.of_int /= /int2bs /mkseq -iotaredE /=.
-rewrite ifF.
- by rewrite /W8.of_int /= /int2bs /mkseq -iotaredE /=.
-rewrite ifF.
- by rewrite /W8.of_int /= /int2bs /mkseq -iotaredE /=.
-rewrite ifF.
- by rewrite /W8.of_int /= /int2bs /mkseq -iotaredE /=.
-rewrite ifT.
- by rewrite /W8.of_int /= /int2bs /mkseq -iotaredE /=.
-have ->: !((of_int 32))%W8.[0].
- by rewrite /W8.of_int /= /int2bs /mkseq -iotaredE /=.
-have ->: !((of_int 32))%W8.[4].
- by rewrite /W8.of_int /= /int2bs /mkseq -iotaredE /=.
-have ->: ((of_int 49))%W8.[0].
- by rewrite /W8.of_int /= /int2bs /mkseq -iotaredE /=.
-have ->: ((of_int 49))%W8.[4].
- by rewrite /W8.of_int /= /int2bs /mkseq -iotaredE /=.
-rewrite !b2i0 !b2i1 /shuffle8 /=.
-move: Ha; rewrite -{1}iotaredE /R2C /= => |> *.
-move: Hb; rewrite -{1}iotaredE /R2C /= => |> *.
-by rewrite -!iotaredE /= /#.
-qed.
-*)
+
 phoare __shuffle8_ph' n _a _b:
  [ Jkem_avx2.M.__shuffle8:
    I16u16_sb n a _a /\ I16u16_sb n b _b
@@ -689,14 +650,6 @@ phoare __shuffle8_ph na nb _a _b:
    ==> I16u16_sb (max na nb) res.`1 (shuffle8 _a _b).`1
        /\ I16u16_sb (max na nb) res.`2 (shuffle8 _a _b).`2 ] = 1%r.
 proof. by conseq __shuffle8_ll (__shuffle8_h na nb _a _b). qed.
-
-(* Do we need this?
-hoare __shuffle8_h _a _b:
- Jkem_avx2.M.__shuffle8:
- a = _a /\ b = _b ==>
- res = (C2R (shuffle8 (R2C _a) (R2C _b)).`1, C2R (shuffle8 (R2C _a) (R2C _b)).`2).
-admitted.
-*)
 
 lemma __shuffle4_ll: islossless Jkem_avx2.M.__shuffle4 by islossless.
 
@@ -840,8 +793,253 @@ op zetas_inv_op = jzetas_inv_exp.
 op flox16_op = jflox16.
 op fhix16_op = jfhix16.
 module Tmp = {
+  proc _ntt (rp:W16.t Array256.t) : W16.t Array256.t = {   
+    var zetasp: W16.t Array400.t;
+    var qx16, vx16: W256.t;
+    var zeta0, zeta1, zeta2, zeta3: W256.t;
+    var r0, r1, r2, r3, r4, r5, r6, r7: W256.t;
+    var i: int;
+    zetasp <- zetas_op;
+    qx16 <- C2R qx16_op;
+    zeta0 <- VPBROADCAST_8u32 (z2u32 zetasp 0);
+    zeta1 <- VPBROADCAST_8u32 (z2u32 zetasp 2);
+    r0 <- P2R rp 0;
+    r1 <- P2R rp 1;
+    r2 <- P2R rp 2;
+    r3 <- P2R rp 3;
+    r4 <- P2R rp 8;
+    r5 <- P2R rp 9;
+    r6 <- P2R rp 10;
+    r7 <- P2R rp 11;
+    (r0, r1, r2, r3, r4, r5, r6, r7) <@ Jkem_avx2.M.__butterfly64x (r0, r1, r2, r3, r4,
+    r5, r6, r7, zeta0, zeta0, zeta1, zeta1, qx16);
+    rp <- PUR rp 0 r0;
+    rp <- PUR rp 1 r1;
+    rp <- PUR rp 2 r2;
+    rp <- PUR rp 3 r3;
+    rp <- PUR rp 8 r4;
+    rp <- PUR rp 9 r5;
+    rp <- PUR rp 10 r6;
+    rp <- PUR rp 11 r7;
+    r0 <- P2R rp 4;
+    r1 <- P2R rp 5;
+    r2 <- P2R rp 6;
+    r3 <- P2R rp 7;
+    r4 <- P2R rp 12;
+    r5 <- P2R rp 13;
+    r6 <- P2R rp 14;
+    r7 <- P2R rp 15;
+    (r0, r1, r2, r3, r4, r5, r6, r7) <@ Jkem_avx2.M.__butterfly64x (r0, r1, r2, r3, r4,
+    r5, r6, r7, zeta0, zeta0, zeta1, zeta1, qx16);
+    rp <- PUR rp 12 r4;
+    rp <- PUR rp 13 r5;
+    rp <- PUR rp 14 r6;
+    rp <- PUR rp 15 r7;
+    i <- 0;
+    while (i < 2) {
+      zeta0 <- VPBROADCAST_8u32 (z2u32 zetasp (4+196*i));
+      zeta1 <- VPBROADCAST_8u32 (z2u32 zetasp (6+196*i));
+      if (i = 0) {
+        r4 <- r0;
+        r5 <- r1;
+        r6 <- r2;
+        r7 <- r3;
+      } else {
+        r4 <- P2R rp (4+8*i);
+        r5 <- P2R rp (5+8*i);
+        r6 <- P2R rp (6+8*i);
+        r7 <- P2R rp (7+8*i);
+      }
+      r0 <- P2R rp (0+8*i);
+      r1 <- P2R rp (1+8*i);
+      r2 <- P2R rp (2+8*i);
+      r3 <- P2R rp (3+8*i);
+      (r0, r1, r2, r3, r4, r5, r6, r7) <@ Jkem_avx2.M.__butterfly64x (r0, r1, r2, r3, r4,
+      r5, r6, r7, zeta0, zeta0, zeta1, zeta1, qx16);
+      zeta0 <- z2u256 zetasp (8+196*i);
+      zeta1 <- z2u256 zetasp (24+196*i);
+      (r0, r4) <@ Jkem_avx2.M.__shuffle8 (r0, r4);
+      (r1, r5) <@ Jkem_avx2.M.__shuffle8 (r1, r5);
+      (r2, r6) <@ Jkem_avx2.M.__shuffle8 (r2, r6);
+      (r3, r7) <@ Jkem_avx2.M.__shuffle8 (r3, r7);
+      (r0, r4, r1, r5, r2, r6, r3, r7) <@ Jkem_avx2.M.__butterfly64x (r0, r4, r1, r5, r2,
+      r6, r3, r7, zeta0, zeta0, zeta1, zeta1, qx16);
+      zeta0 <- z2u256 zetasp (40+196*i);
+      zeta1 <- z2u256 zetasp (56+196*i);
+      (r0, r2) <@ Jkem_avx2.M.__shuffle4 (r0, r2);
+      (r4, r6) <@ Jkem_avx2.M.__shuffle4 (r4, r6);
+      (r1, r3) <@ Jkem_avx2.M.__shuffle4 (r1, r3);
+      (r5, r7) <@ Jkem_avx2.M.__shuffle4 (r5, r7);
+      (r0, r2, r4, r6, r1, r3, r5, r7) <@ Jkem_avx2.M.__butterfly64x (r0, r2, r4, r6, r1,
+      r3, r5, r7, zeta0, zeta0, zeta1, zeta1, qx16);
+      zeta0 <- z2u256 zetasp (72+196*i);
+      zeta1 <- z2u256 zetasp (88+196*i);
+      (r0, r1) <@ Jkem_avx2.M.__shuffle2 (r0, r1);
+      (r2, r3) <@ Jkem_avx2.M.__shuffle2 (r2, r3);
+      (r4, r5) <@ Jkem_avx2.M.__shuffle2 (r4, r5);
+      (r6, r7) <@ Jkem_avx2.M.__shuffle2 (r6, r7);
+      (r0, r1, r2, r3, r4, r5, r6, r7) <@ Jkem_avx2.M.__butterfly64x (r0, r1, r2, r3, r4,
+      r5, r6, r7, zeta0, zeta0, zeta1, zeta1, qx16);
+      zeta0 <- z2u256 zetasp (104+196*i);
+      zeta1 <- z2u256 zetasp (120+196*i);
+      (r0, r4) <@ Jkem_avx2.M.__shuffle1 (r0, r4);
+      (r1, r5) <@ Jkem_avx2.M.__shuffle1 (r1, r5);
+      (r2, r6) <@ Jkem_avx2.M.__shuffle1 (r2, r6);
+      (r3, r7) <@ Jkem_avx2.M.__shuffle1 (r3, r7);
+      (r0, r4, r1, r5, r2, r6, r3, r7) <@ Jkem_avx2.M.__butterfly64x (r0, r4, r1, r5, r2,
+      r6, r3, r7, zeta0, zeta0, zeta1, zeta1, qx16);
+      zeta0 <- z2u256 zetasp (136+196*i);
+      zeta1 <- z2u256 zetasp (168+196*i);
+      zeta2 <- z2u256 zetasp (152+196*i);
+      zeta3 <- z2u256 zetasp (184+196*i);
+      (r0, r4, r2, r6, r1, r5, r3, r7) <@ Jkem_avx2.M.__butterfly64x (r0, r4, r2, r6, r1,
+      r5, r3, r7, zeta0, zeta1, zeta2, zeta3, qx16);
+      vx16 <- C2R vx16_op;
+      r0 <@ Jkem_avx2.M.__red16x (r0, qx16, vx16);
+      r4 <@ Jkem_avx2.M.__red16x (r4, qx16, vx16);
+      r2 <@ Jkem_avx2.M.__red16x (r2, qx16, vx16);
+      r6 <@ Jkem_avx2.M.__red16x (r6, qx16, vx16);
+      r1 <@ Jkem_avx2.M.__red16x (r1, qx16, vx16);
+      r5 <@ Jkem_avx2.M.__red16x (r5, qx16, vx16);
+      r3 <@ Jkem_avx2.M.__red16x (r3, qx16, vx16);
+      r7 <@ Jkem_avx2.M.__red16x (r7, qx16, vx16);
+      rp <- PUR rp (0+8*i) r0;
+      rp <- PUR rp (1+8*i) r4;
+      rp <- PUR rp (2+8*i) r1;
+      rp <- PUR rp (3+8*i) r5;
+      rp <- PUR rp (4+8*i) r2;
+      rp <- PUR rp (5+8*i) r6;
+      rp <- PUR rp (6+8*i) r3;
+      rp <- PUR rp (7+8*i) r7;
+      i <- i + 1;
+    }
+    return (rp);
+  }
+  proc _invntt (rp:W16.t Array256.t) : W16.t Array256.t = {
+    var zetasp: W16.t Array400.t;
+    var qx16, vx16, flox16, fhix16: W256.t;
+    var i: int;
+    var zeta0, zeta1, zeta2, zeta3: W256.t;
+    var r0, r1, r2, r3, r4, r5, r6, r7: W256.t;
+    zetasp <- zetas_inv_op;
+    qx16 <- C2R qx16_op;
+    i <- 0;
+    while (i < 2) {
+      zeta0 <- z2u256 zetasp (0 + (196 * i));
+      zeta2 <- z2u256 zetasp (16 + (196 * i));
+      zeta1 <- z2u256 zetasp (32 + (196 * i));
+      zeta3 <- z2u256 zetasp (48 + (196 * i));
+      r0 <- P2R rp (0+8*i);
+      r1 <- P2R rp (1+8*i);
+      r2 <- P2R rp (2+8*i);
+      r3 <- P2R rp (3+8*i);
+      r4 <- P2R rp (4+8*i);
+      r5 <- P2R rp (5+8*i);
+      r6 <- P2R rp (6+8*i);
+      r7 <- P2R rp (7+8*i);
+      (r0, r1, r4, r5, r2, r3, r6, r7) <@ Jkem_avx2.M.__invntt___butterfly64x (r0, r1,
+      r4, r5, r2, r3, r6, r7, zeta0, zeta1, zeta2, zeta3, qx16);
+      (* 4 4 1 1 4 4 1 1 *)
+      vx16 <- C2R vx16_op;
+      zeta0 <- z2u256 zetasp (64 + (196 * i));
+      zeta1 <- z2u256 zetasp (80 + (196 * i));
+      (r0, r1, r2, r3, r4, r5, r6, r7) <@ Jkem_avx2.M.__invntt___butterfly64x (r0, r1,
+      r2, r3, r4, r5, r6, r7, zeta0, zeta0, zeta1, zeta1, qx16);
+      (* 8 8 2 2 1 1 1 1 *)
+      r0 <@ Jkem_avx2.M.__red16x (r0, qx16, vx16);
+      r1 <@ Jkem_avx2.M.__red16x (r1, qx16, vx16);      
+      (r0, r1) <@ Jkem_avx2.M.__shuffle1 (r0, r1);
+      (r2, r3) <@ Jkem_avx2.M.__shuffle1 (r2, r3);
+      (r4, r5) <@ Jkem_avx2.M.__shuffle1 (r4, r5);
+      (r6, r7) <@ Jkem_avx2.M.__shuffle1 (r6, r7);
+      zeta0 <- z2u256 zetasp (96 + (196 * i));
+      zeta1 <- z2u256 zetasp (112 + (196 * i));
+      (r0, r2, r4, r6, r1, r3, r5, r7) <@ Jkem_avx2.M.__invntt___butterfly64x (r0, r2,
+      r4, r6, r1, r3, r5, r7, zeta0, zeta0, zeta1, zeta1, qx16);
+      (*.4 1 4 1 2 1 2 1 *)
+      (r0, r2) <@ Jkem_avx2.M.__shuffle2 (r0, r2);
+      (r4, r6) <@ Jkem_avx2.M.__shuffle2 (r4, r6);
+      (r1, r3) <@ Jkem_avx2.M.__shuffle2 (r1, r3);
+      (r5, r7) <@ Jkem_avx2.M.__shuffle2 (r5, r7);
+      zeta0 <- z2u256 zetasp (128 + (196 * i));
+      zeta1 <- z2u256 zetasp (144 + (196 * i));
+      (r0, r4, r1, r5, r2, r6, r3, r7) <@ Jkem_avx2.M.__invntt___butterfly64x (r0, r4,
+      r1, r5, r2, r6, r3, r7, zeta0, zeta0, zeta1, zeta1, qx16);
+      (* 8 2 1 1 4 2 1 1 *)
+      r0 <@ Jkem_avx2.M.__red16x (r0, qx16, vx16);
+      (r0, r4) <@ Jkem_avx2.M.__shuffle4 (r0, r4);
+      (r1, r5) <@ Jkem_avx2.M.__shuffle4 (r1, r5);
+      (r2, r6) <@ Jkem_avx2.M.__shuffle4 (r2, r6);
+      (r3, r7) <@ Jkem_avx2.M.__shuffle4 (r3, r7);
+      zeta0 <- z2u256 zetasp (160 + (196 * i));
+      zeta1 <- z2u256 zetasp (176 + (196 * i));
+      (r0, r1, r2, r3, r4, r5, r6, r7) <@ Jkem_avx2.M.__invntt___butterfly64x (r0, r1,
+      r2, r3, r4, r5, r6, r7, zeta0, zeta0, zeta1, zeta1, qx16);
+      (* 8 4 2 2 1 1 1 1 *)
+      r0 <@ Jkem_avx2.M.__red16x (r0, qx16, vx16);
+      (r0, r1) <@ Jkem_avx2.M.__shuffle8 (r0, r1);
+      (r2, r3) <@ Jkem_avx2.M.__shuffle8 (r2, r3);
+      (r4, r5) <@ Jkem_avx2.M.__shuffle8 (r4, r5);
+      (r6, r7) <@ Jkem_avx2.M.__shuffle8 (r6, r7);
+      zeta0 <- VPBROADCAST_8u32 (z2u32 zetasp (192 + (196 * i)));
+      zeta1 <- VPBROADCAST_8u32 (z2u32 zetasp (194 + (196 * i)));
+      (r0, r2, r4, r6, r1, r3, r5, r7) <@ Jkem_avx2.M.__invntt___butterfly64x (r0, r2,
+      r4, r6, r1, r3, r5, r7, zeta0, zeta0, zeta1, zeta1, qx16);
+      (* 8 1 4 1 2 1 2 1 *)
+      r0 <@ Jkem_avx2.M.__red16x (r0, qx16, vx16);
+      if (i = 0) {
+      rp <- PUR rp (0+8*i) r0; (* 2 *)
+      rp <- PUR rp (1+8*i) r2; (* 4 *)
+      rp <- PUR rp (2+8*i) r4; (* 2 *)
+      rp <- PUR rp (3+8*i) r6; (* 2 *)
+      }
+      rp <- PUR rp (4+8*i) r1; (* 1 *)
+      rp <- PUR rp (5+8*i) r3; (* 1 *)
+      rp <- PUR rp (6+8*i) r5; (* 1 *)
+      rp <- PUR rp (7+8*i) r7; (* 1 *)
+      i <- i + 1;
+    }
+    zeta0 <- VPBROADCAST_8u32 (z2u32 zetasp 392);
+    zeta1 <- VPBROADCAST_8u32 (z2u32 zetasp 394);
+    flox16 <- C2R flox16_op;
+    fhix16 <- C2R fhix16_op;
+    i <- 0;
+    while (i < 2) {
+      if (i = 0) {
+        r7 <- r6;
+        r6 <- r4;
+        r5 <- r2;
+        r4 <- r0;
+      } else {
+        r4 <- P2R rp (8+4*i); (* 2 *)
+        r5 <- P2R rp (9+4*i); (* 4 *)
+        r6 <- P2R rp (10+4*i); (* 2 *)
+        r7 <- P2R rp (11+4*i); (* 2 *)
+      }
+      r0 <- P2R rp (0+4*i); (* 2 *)
+      r1 <- P2R rp (1+4*i); (* 4 *)
+      r2 <- P2R rp (2+4*i); (* 2 *)
+      r3 <- P2R rp (3+4*i); (* 2 *)
+      (r0, r1, r2, r3, r4, r5, r6, r7) <@ Jkem_avx2.M.__invntt___butterfly64x (r0, r1,
+        r2, r3, r4, r5, r6, r7, zeta0, zeta0, zeta1, zeta1, qx16);
+      (* 4 8 4 4 1 1 1 1 *)
+      rp <- PUR rp (8+4*i) r4;
+      rp <- PUR rp (9+4*i) r5;
+      rp <- PUR rp (10+4*i) r6;
+      rp <- PUR rp (11+4*i) r7;
+      r0 <@ Jkem_avx2.M.__fqmulprecomp16x (r0, flox16, fhix16, qx16);
+      r1 <@ Jkem_avx2.M.__fqmulprecomp16x (r1, flox16, fhix16, qx16);
+      r2 <@ Jkem_avx2.M.__fqmulprecomp16x (r2, flox16, fhix16, qx16);
+      r3 <@ Jkem_avx2.M.__fqmulprecomp16x (r3, flox16, fhix16, qx16);
+      rp <- PUR rp (0+4*i) r0;
+      rp <- PUR rp (1+4*i) r1;
+      rp <- PUR rp (2+4*i) r2;
+      rp <- PUR rp (3+4*i) r3;
+      i <- i + 1;
+    }
+    return (rp);
+  }
   proc __ntt_level0 (rp:W16.t Array256.t) : W16.t Array256.t = {
-    
     var zetasp:W16.t Array400.t;
     var qx16:W256.t;
     var zeta0:W256.t;
@@ -857,10 +1055,8 @@ module Tmp = {
     zetasp <- witness;
     zetasp <- zetas_op;
     qx16 <- C2R qx16_op;
-    zeta0 <-
-    VPBROADCAST_8u32 (z2u32 zetasp 0);
-    zeta1 <-
-    VPBROADCAST_8u32 (z2u32 zetasp 2);
+    zeta0 <- VPBROADCAST_8u32 (z2u32 zetasp 0);
+    zeta1 <- VPBROADCAST_8u32 (z2u32 zetasp 2);
     r0 <- P2R rp 0;
     r1 <- P2R rp 1;
     r2 <- P2R rp 2;
@@ -900,8 +1096,6 @@ module Tmp = {
     return (rp);
   }
   proc __ntt_level1t6 (rp:W16.t Array256.t) : W16.t Array256.t = {
-    var aux: int;
-    
     var zetasp:W16.t Array400.t;
     var qx16:W256.t;
     var i:int;
@@ -995,99 +1189,6 @@ module Tmp = {
     return (rp);
   }
   proc __invntt_levels0t5 (rp:W16.t Array256.t) : W16.t Array256.t = {
-    var aux: int;
-    
-    var zetasp:W16.t Array400.t;
-    var qx16:W256.t;
-    var i:int;
-    var zeta0:W256.t;
-    var zeta1:W256.t;
-    var zeta2:W256.t;
-    var zeta3:W256.t;
-    var r0:W256.t;
-    var r1:W256.t;
-    var r2:W256.t;
-    var r3:W256.t;
-    var r4:W256.t;
-    var r5:W256.t;
-    var r6:W256.t;
-    var r7:W256.t;
-    var vx16:W256.t;
-    zetasp <- witness;
-    zetasp <- zetas_inv_op;
-    qx16 <- C2R qx16_op;
-    i <- 0;
-    while (i < 2) {
-      zeta0 <- z2u256 zetasp (0 + (196 * i));
-      zeta1 <- z2u256 zetasp (32 + (196 * i));
-      zeta2 <- z2u256 zetasp (16 + (196 * i));
-      zeta3 <- z2u256 zetasp (48 + (196 * i));
-      r0 <- P2R rp (0+8*i);
-      r1 <- P2R rp (1+8*i);
-      r2 <- P2R rp (2+8*i);
-      r3 <- P2R rp (3+8*i);
-      r4 <- P2R rp (4+8*i);
-      r5 <- P2R rp (5+8*i);
-      r6 <- P2R rp (6+8*i);
-      r7 <- P2R rp (7+8*i);
-      (r0, r1, r4, r5, r2, r3, r6, r7) <@ Jkem_avx2.M.__invntt___butterfly64x (r0, r1,
-      r4, r5, r2, r3, r6, r7, zeta0, zeta1, zeta2, zeta3, qx16);
-      zeta0 <- z2u256 zetasp (64 + (196 * i));
-      zeta1 <- z2u256 zetasp (80 + (196 * i));
-      (r0, r1, r2, r3, r4, r5, r6, r7) <@ Jkem_avx2.M.__invntt___butterfly64x (r0, r1,
-      r2, r3, r4, r5, r6, r7, zeta0, zeta0, zeta1, zeta1, qx16);
-      (r0, r1) <@ Jkem_avx2.M.__shuffle1 (r0, r1);
-      (r2, r3) <@ Jkem_avx2.M.__shuffle1 (r2, r3);
-      (r4, r5) <@ Jkem_avx2.M.__shuffle1 (r4, r5);
-      (r6, r7) <@ Jkem_avx2.M.__shuffle1 (r6, r7);
-      zeta0 <- z2u256 zetasp (96 + (196 * i));
-      zeta1 <- z2u256 zetasp (112 + (196 * i));
-      vx16 <- C2R vx16_op;
-      (r0, r2, r4, r6, r1, r3, r5, r7) <@ Jkem_avx2.M.__invntt___butterfly64x (r0, r2,
-      r4, r6, r1, r3, r5, r7, zeta0, zeta0, zeta1, zeta1, qx16);
-      r0 <@ Jkem_avx2.M.__red16x (r0, qx16, vx16);
-      (r0, r2) <@ Jkem_avx2.M.__shuffle2 (r0, r2);
-      (r4, r6) <@ Jkem_avx2.M.__shuffle2 (r4, r6);
-      (r1, r3) <@ Jkem_avx2.M.__shuffle2 (r1, r3);
-      (r5, r7) <@ Jkem_avx2.M.__shuffle2 (r5, r7);
-      zeta0 <- z2u256 zetasp (128 + (196 * i));
-      zeta1 <- z2u256 zetasp (144 + (196 * i));
-      (r0, r4, r1, r5, r2, r6, r3, r7) <@ Jkem_avx2.M.__invntt___butterfly64x (r0, r4,
-      r1, r5, r2, r6, r3, r7, zeta0, zeta0, zeta1, zeta1, qx16);
-      r0 <@ Jkem_avx2.M.__red16x (r0, qx16, vx16);
-      (r0, r4) <@ Jkem_avx2.M.__shuffle4 (r0, r4);
-      (r1, r5) <@ Jkem_avx2.M.__shuffle4 (r1, r5);
-      (r2, r6) <@ Jkem_avx2.M.__shuffle4 (r2, r6);
-      (r3, r7) <@ Jkem_avx2.M.__shuffle4 (r3, r7);
-      zeta0 <- z2u256 zetasp (160 + (196 * i));
-      zeta1 <- z2u256 zetasp (176 + (196 * i));
-      (r0, r1, r2, r3, r4, r5, r6, r7) <@ Jkem_avx2.M.__invntt___butterfly64x (r0, r1,
-      r2, r3, r4, r5, r6, r7, zeta0, zeta0, zeta1, zeta1, qx16);
-      r0 <@ Jkem_avx2.M.__red16x (r0, qx16, vx16);
-      (r0, r1) <@ Jkem_avx2.M.__shuffle8 (r0, r1);
-      (r2, r3) <@ Jkem_avx2.M.__shuffle8 (r2, r3);
-      (r4, r5) <@ Jkem_avx2.M.__shuffle8 (r4, r5);
-      (r6, r7) <@ Jkem_avx2.M.__shuffle8 (r6, r7);
-      zeta0 <- VPBROADCAST_8u32 (z2u32 zetasp (192 + (196 * i)));
-      zeta1 <- VPBROADCAST_8u32 (z2u32 zetasp (194 + (196 * i)));
-      (r0, r2, r4, r6, r1, r3, r5, r7) <@ Jkem_avx2.M.__invntt___butterfly64x (r0, r2,
-      r4, r6, r1, r3, r5, r7, zeta0, zeta0, zeta1, zeta1, qx16);
-      r0 <@ Jkem_avx2.M.__red16x (r0, qx16, vx16);
-      rp <- PUR rp (0+8*i) r0;
-      rp <- PUR rp (1+8*i) r2;
-      rp <- PUR rp (2+8*i) r4;
-      rp <- PUR rp (3+8*i) r6;
-      rp <- PUR rp (4+8*i) r1;
-      rp <- PUR rp (5+8*i) r3;
-      rp <- PUR rp (6+8*i) r5;
-      rp <- PUR rp (7+8*i) r7;
-      i <- i + 1;
-    }
-    return (rp);
-  }
-  proc __invntt_levels0t5ALT (rp:W16.t Array256.t) : W16.t Array256.t = {
-    var aux: int;
-    
     var zetasp:W16.t Array400.t;
     var qx16:W256.t;
     var i:int;
@@ -1238,11 +1339,6 @@ module Tmp = {
     }
     return (rp);
   }
-  proc _poly_invntt (rp:W16.t Array256.t) : W16.t Array256.t = {
-    rp <@ __invntt_levels0t5 (rp);
-    rp <@ __invntt_level6 (rp);
-    return (rp);
-  }
 
   proc __schoolbookx16(are aim bre bim zetas zetasqinv qx16 qinvx16: W256.t, sign: int): W256.t*W256.t = {
    return witness;
@@ -1331,11 +1427,12 @@ module Tmp = {
 
 }.
 
-equiv __ntt_level0_eq_:
- Jkem_avx2.M.__ntt_level0 ~ Tmp.__ntt_level0:
+equiv __ntt_eq_:
+ Jkem_avx2.M._poly_ntt ~ Tmp._ntt:
  ={rp} ==> ={res}.
+proof.
 proc.
-seq 13 13: (={rp,r0,r1,r2,r3,r4,r5,r6,r7,zeta0,zeta1,qx16}).
+seq 13 12: (={rp,r0,r1,r2,r3,r4,r5,r6,r7,zetasp,zeta0,zeta1,qx16}).
  by wp; skip; rewrite !P2RE //. 
 seq 1 1: #pre.
  by sim.
@@ -1343,107 +1440,93 @@ seq 16 16: #pre.
  by wp; skip => />; rewrite !P2RE // !PURE //.
 seq 1 1: #pre.
  by sim.
-by wp; skip => />; rewrite !PURE //.
-qed.
-
-equiv __ntt_level1t6_eq_:
- Jkem_avx2.M.__ntt_level1t6 ~ Tmp.__ntt_level1t6:
- ={rp} ==> ={res}.
-proc.
-seq 3 3: (={zetasp,qx16,rp}).
- by auto => />.
-while (0 <= i{2} /\ ={i,zetasp,qx16,rp}).
- seq 10 10: (#pre /\ ={zeta0,zeta1,r0,r1,r2,r3,r4,r5,r6,r7}).
+seq 5 5: (0 <= i{2} /\ ={i} /\ #pre).
+ by wp; skip => />; rewrite !PURE //.
+while (#pre).
+ seq 7 7: (#pre).
   by auto => /> *; rewrite !P2RE /#.
  seq 1 1: (#pre).
   by conseq />; sim.
- seq 6 6: (#pre).
-  conseq |>; sim; auto => |> *.
-  by rewrite /z2u256 !mulrDr !mulrA /=.
+ seq 2 2: (#pre).
+  by auto => /> *; rewrite /z2u256 !mulrDr !mulrA /=.
+ seq 5 5: (#pre).
+  by conseq />; sim.
+ seq 2 2: (#pre).
+  by auto => /> *; rewrite /z2u256 !mulrDr !mulrA /=.
+ seq 5 5: (#pre).
+  by conseq />; sim.
+ seq 2 2: (#pre).
+  by auto => /> *; rewrite /z2u256 !mulrDr !mulrA /=.
+ seq 5 5: (#pre).
+  by conseq />; sim.
+ seq 2 2: (#pre).
+  by auto => /> *; rewrite /z2u256 !mulrDr !mulrA /=.
+ seq 5 5: (#pre).
+  by conseq />; sim.
+ seq 4 4: (={zeta2,zeta3} /\ #pre).
+  by auto => /> *; rewrite /z2u256 !mulrDr !mulrA /=.
  seq 1 1: (#pre).
   by conseq />; sim.
- seq 6 6: (#pre).
-  conseq />; sim; auto => /> *.
-  by rewrite /z2u256 !mulrDr !mulrA /=.
- seq 1 1: (#pre).
+ seq 1 1: (={vx16} /\ #pre).
+  by wp; skip; rewrite /C2R /vx16_op /#.
+ seq 8 8: (#pre).
   by conseq />; sim.
- seq 6 6: (#pre).
-  conseq />; sim; auto => /> *.
-  by rewrite /z2u256 !mulrDr !mulrA /=.
- seq 1 1: (#pre).
-  by conseq />; sim.
- seq 6 6: (#pre).
-  conseq />; sim; auto => /> *.
-  by rewrite /z2u256 !mulrDr !mulrA /=.
- seq 1 1: (#pre).
-  by conseq />; sim.
- seq 4 4: (#pre /\ ={zeta2,zeta3}).
-  auto => /> *.
-  by rewrite /z2u256 !mulrDr !mulrA /=.
- seq 10 10: (#pre).
-  conseq />; sim.
-  auto => />.
-  by sim.
- by auto => /> *; rewrite !PURE 1..8:/# !mulrDr !mulrA /= /#.
+ by wp; skip => |> *; rewrite !PURE 1..8:/# !mulrDr !mulrA /= /#.
 by auto => />.
 qed.
 
-equiv __invntt_levels0t5_eq_:
- Jkem_avx2.M.__invntt_levels0t5 ~ Tmp.__invntt_levels0t5ALT:
+
+equiv __invntt_eq_:
+ Jkem_avx2.M._poly_invntt ~ Tmp._invntt:
  ={rp} ==> ={res}.
 proof.
-admit (*
-(* OBS: change implementation!!! *)
 proc.
-seq 3 3: (={zetasp,qx16,rp}).
- by auto => />.
-while (0 <= i{2} /\ ={i,zetasp,qx16,rp}).
- seq 12 12: (#pre /\ ={zeta0,zeta1,zeta2,zeta3,r0,r1,r2,r3,r4,r5,r6,r7}).
-  by auto => /> *; rewrite !P2RE /#.
- seq 1 1: (#pre).
+seq 4 3: (i{2}=0 /\ ={i,rp,zetasp,qx16}).
+ by wp; skip; rewrite /C2R //.
+seq 6 6: (#pre /\ ={r0,r2,r4,r6,zeta0,zeta1,flox16,fhix16}).
+ wp; while (0 <= i{2} /\ #[/2:]pre /\ (i{2}=0 \/ ={r0,r2,r4,r6})).
+  seq 12 12: (i{2} < 2 /\ #[/:5]pre /\ ={r0,r1,r2,r3,r4,r5,r6,r7,zeta0,zeta1,zeta2,zeta3}).
+   by auto => /> *; rewrite /z2u256 !mulrDr !mulrA !P2RE /#.
+  seq 1 1: (#pre).
+   by conseq />; sim.
+  seq 3 3: (#pre /\ ={vx16}).
+   by auto => /> *; rewrite /z2u256 !mulrDr !mulrA /#.
+  seq 7 7: (#pre).
+   by conseq />; sim.
+  seq 2 2: (#pre).
+   by auto => /> *; rewrite /z2u256 !mulrDr !mulrA /#.
+  seq 5 5: (#pre).
+   by conseq />; sim.
+  seq 2 2: (#pre).
+   by auto => /> *; rewrite /z2u256 !mulrDr !mulrA /#.
+  seq 6 6: (#pre).
+   by conseq />; sim.
+  seq 2 2: (#pre).
+   by auto => /> *; rewrite /z2u256 !mulrDr !mulrA /#.
+  seq 6 6: (#pre).
+   by conseq />; sim.
+  seq 2 2: (#pre).
+   by auto => /> *; rewrite /z2u32 /#. 
+  seq 2 2: (#pre).
+   by conseq />; sim.
+  if => //.
+   by wp; skip => /> *; rewrite !PURE 1..8:/# /= /#.
+  by wp; skip => /> *; rewrite !PURE 1..4:/# /= !mulrDr !mulrA /= /#.
+ by auto => /> * /#.
+while (#[/2:]pre /\ 0 <= i{2}).
+ seq 5 5: (={r1,r3,r5,r7} /\ #pre).
+  if => //.
+   by wp; skip => /> *; rewrite !P2RE /#. 
+  by wp; skip => /> *; rewrite !P2RE /#. 
+ seq 1 1: (#pre).   
   by conseq />; sim.
- seq 7 7: (#pre).
-  conseq |>; sim; auto => |> *.
-  by rewrite /z2u256 !mulrDr !mulrA /=.
- seq 9 9: (#pre /\ ={vx16}).
-  conseq |>; sim; auto => |> *.
-  by rewrite /z2u256 !mulrDr !mulrA /=.
- seq 8 8: (#pre).
-  conseq |>; sim; auto => |> *.
-  by rewrite /z2u256 !mulrDr !mulrA /=.
- seq 8 8: (#pre).
-  conseq |>; sim; auto => |> *.
-  by rewrite /z2u256 !mulrDr !mulrA /=.
  seq 4 4: (#pre).
-  conseq |>; sim; auto => |> *.
-  by rewrite /z2u32 !mulrDr !mulrA /=.
- by auto => /> *; rewrite !PURE 1..8:/# !mulrDr !mulrA /= /#.
-by auto => />.
-*).
+  by wp; skip => /> *; rewrite /C2R !PURE /#. 
+ seq 4 4: (#pre).   
+  by conseq />; sim.
+ by wp; skip => /> *; rewrite !PURE /#. 
+by auto.
 qed.
-
-equiv __invntt_level6_eq_:
- Jkem_avx2.M.__invntt_level6 ~ Tmp.__invntt_level6:
- ={rp} ==> ={res}.
-proc.
-seq 5 5: (={zeta0,zeta1,qx16,rp}).
- by auto => />.
-while (0 <= i{2} /\ ={i,zeta0,zeta1,qx16,rp}).
- seq 8 8: (#pre /\ ={r0,r1,r2,r3,r4,r5,r6,r7}).
-  by auto => /> *; rewrite !P2RE /#.
- seq 3 3: (#pre /\ ={flox16,fhix16}).
-  conseq |>; sim; auto => |> *.
-  by conseq |>; sim.
- seq 8 8: (#pre).
-  conseq |>; sim; auto => |> *.
-  by rewrite !PURE /#.
- by auto => /> *; rewrite !PURE 1..4:/# !mulrDr !mulrA /= /#.
-by auto => />.
-qed. 
-
-
-
-
 
 lemma Iu16_ub_of_int n:
  0 <= n < 3329 =>
@@ -1451,50 +1534,19 @@ lemma Iu16_ub_of_int n:
 proof. by move=> /> *; rewrite of_sintK smod_small /#. qed.
 
 
-
-equiv __ntt_level0_eq:
- NTT_AVX.__ntt_level0 ~ Jkem_avx2.M.__ntt_level0:
- I256u16_sb (2*q) rp{2} rp{1} ==> I256u16_sb (3*q) res{2} res{1}.
+equiv _poly_ntt_eq:
+ NTT_AVX.ntt ~Jkem_avx2.M._poly_ntt:
+ rp{1}=lift_array256 rp{2} /\ signed_bound_cxq rp{2} 0 256 2 ==>
+ res{1}=lift_array256 res{2} /\
+ pos_bound256_cxq res{2} 0 256 2.
 proof.
-transitivity Tmp.__ntt_level0
- ( I256u16_sb (2*q) rp{2} rp{1} ==> I256u16_sb (3*q) res{2} res{1} )
- ( ={rp} ==> ={res} );
-  last by symmetry; conseq __ntt_level0_eq_.
-  by move=> |> &1 &2 H; exists arg{2}. 
- done.
-proc; simplify.
-inline NTT_AVX.__ntt_level0.
-wp; call (butterfly64x_eq (2*q)); simplify.
-wp; call (butterfly64x_eq (2*q)); simplify.
-wp; skip => &1 &2 Hpre qx16 z0R z1R z1L.
-have ->: 2 * q + q <= 32767 by smt().
-have ->: qinv16u16M z0R z1R.
- by rewrite /z0R /z1R /zR !z2u32E //= /VPBROADCAST_8u32 /qinv16u16M -iotaredE /= !R2C_pack16 //=. 
-have ->: x16_spec q qx16.
- by rewrite x16_spec_C2R /q /=.
-have ->: I16u16M_ub q z1R z1L.
- by move: Iu16_ub_of_int; rewrite /z1L /z1R /zR /zetas_op !z2u32E //= /VPBROADCAST_8u32 /R2C -iotaredE /= -inFqM_mod /q /= !Iu16_ub_of_int.
-move: Hpre; rewrite -{2}iotaredE /= => |> *.
-rewrite (P2RS rp{2}) /= !PUR_i //= !P2R_i //= => |> *.
-rewrite (P2RS rp{2}) /= !PUR_i //= => |> *.
-have E: 2*q+q = 3*q by ring.
-by rewrite -{2}iotaredE /= !P2R_i //= !P2C_i //= -!E. 
-qed.
-
-equiv __ntt_level1t6_eq:
- NTT_AVX.__ntt_level1t6 ~ Jkem_avx2.M.__ntt_level1t6:
- I256u16_sb (3*q) rp{2} rp{1} ==> I256u16_ub (2*q) res{2} res{1}.
-proof.
-transitivity Tmp.__ntt_level1t6
- ( I256u16_sb (3*q) rp{2} rp{1} ==> I256u16_ub (2*q) res{2} res{1} )
- ( ={rp} ==> ={res} );
-  last by symmetry; conseq __ntt_level1t6_eq_.
-  move => &1 &2 *; exists arg{2}; smt().
- done.
+transitivity Tmp._ntt
+ ( I256u16_sb (2*q) rp{2} rp{1} ==> I256u16_ub (2*q) res{2} res{1} )
+ ( ={rp} ==> ={res} ); last by symmetry; conseq __ntt_eq_.
+  by move=> |> &2 H; exists arg{2}; rewrite I256u16_sbE. 
+ by move => &1 &m &2 /= ??; rewrite -I256u16_ubE /#.
 proc.
-unroll {2} 5; rcondt {2} 5.
- by move=> &m; wp;skip => /=.
-seq 10 15: (i{2} = 0 /\ zetasp{2}=zetas_op  /\ x16_spec q qx16{2} /\
+seq 6 35: (x16_spec q qx16{2} /\ zetasp{2}=zetas_op  /\ i{2}=0 /\
   I16u16_sb (3*q) (P2R rp{2} 8) (P2C rp{1} 8) /\
   I16u16_sb (3*q) (P2R rp{2} 9) (P2C rp{1} 9) /\
   I16u16_sb (3*q) (P2R rp{2} 10) (P2C rp{1} 10) /\
@@ -1503,6 +1555,33 @@ seq 10 15: (i{2} = 0 /\ zetasp{2}=zetas_op  /\ x16_spec q qx16{2} /\
   I16u16_sb (3*q) (P2R rp{2} 13) (P2C rp{1} 13) /\
   I16u16_sb (3*q) (P2R rp{2} 14) (P2C rp{1} 14) /\
   I16u16_sb (3*q) (P2R rp{2} 15) (P2C rp{1} 15) /\
+  I16u16_sb (3*q) (P2R rp{2} 0) (P2C rp{1} 0) /\
+  I16u16_sb (3*q) (P2R rp{2} 1) (P2C rp{1} 1) /\
+  I16u16_sb (3*q) (P2R rp{2} 2) (P2C rp{1} 2) /\
+  I16u16_sb (3*q) (P2R rp{2} 3) (P2C rp{1} 3) /\
+  I16u16_sb (3*q) r0{2} (P2C rp{1} 4) /\
+  I16u16_sb (3*q) r1{2} (P2C rp{1} 5) /\
+  I16u16_sb (3*q) r2{2} (P2C rp{1} 6) /\
+  I16u16_sb (3*q) r3{2} (P2C rp{1} 7)).
+ wp; call (butterfly64x_eq (2*q)).
+ wp; call (butterfly64x_eq (2*q)).
+ wp; skip => &1 &2 Hpre qx16 z0R z1R /=.
+ have ->: 2 * q + q <= 32767 by smt().
+ have ->: qinv16u16M z0R z1R.
+  by rewrite /z0R /z1R /zR !z2u32E //= /VPBROADCAST_8u32 /qinv16u16M -iotaredE /= !R2C_pack16 //=. 
+ have ->: x16_spec q qx16.
+  by rewrite x16_spec_C2R /q /=.
+ pose z1L:= Array16.init _.
+ have ->: I16u16M_ub q z1R z1L.
+  by move: Iu16_ub_of_int; rewrite /z1L /z1R /zR /zetas_op !z2u32E //= /VPBROADCAST_8u32 /R2C -iotaredE /= -inFqM_mod /q /= !Iu16_ub_of_int.
+ move: Hpre; rewrite -{2}iotaredE /= => |> *.
+ rewrite (P2RS rp{2}) /= !PUR_i //= !P2R_i //= => |> *.
+ rewrite (P2RS rp{2}) /= !PUR_i //= => |> *.
+ have E: 2*q+q = 3*q by ring.
+ by rewrite -!E !P2R_i 1..40:// !P2C_i //.
+unroll {2} 1; rcondt {2} 1.
+ by move=> &m; skip => /=.
+seq 10 8: (#[/:11]pre /\
   I16u16_sb (4*q) r0{2} r0a{1} /\
   I16u16_sb (4*q) r1{2} r1a{1} /\
   I16u16_sb (4*q) r2{2} r2a{1} /\
@@ -1511,17 +1590,15 @@ seq 10 15: (i{2} = 0 /\ zetasp{2}=zetas_op  /\ x16_spec q qx16{2} /\
   I16u16_sb (4*q) r5{2} r5a{1} /\
   I16u16_sb (4*q) r6{2} r6a{1} /\
   I16u16_sb (4*q) r7{2} r7a{1} ).
- wp; call (butterfly64x_eq (3*q)); wp; skip => &1 &2 Hpre qx16 z0R z1R |>.
+ wp; call (butterfly64x_eq (3*q)); wp; skip => &1 &2 Hpre z0R z1R |>.
+ move: Hpre => |> *.
  have ->:  3 * q + q <= 32767 by rewrite /q.
  have ->: qinv16u16M z0R z1R.
-  by rewrite /z0R /z1R /zR !z2u32E 1..2://= /VPBROADCAST_8u32 /qinv16u16M -iotaredE /=.
- have ->: x16_spec q qx16.
-  by rewrite x16_spec_C2R /q /=.
+  by rewrite /z0R /z1R /zetas_op !z2u32E 1..2:/# /VPBROADCAST_8u32 /qinv16u16M -iotaredE /= !R2C_pack16 //=.
  pose z1L:= Array16.init _.
  have ->: I16u16M_ub q z1R z1L.
   by move: Iu16_ub_of_int; rewrite /z1L /z1R /zR /zetas_op !z2u32E //= /VPBROADCAST_8u32 /R2C -iotaredE /= -inFqM_mod /q /= !Iu16_ub_of_int.
- have E: 3*q+q = 4*q by ring.
- by move: Hpre; rewrite -{2}iotaredE /= !E => |> *.
+ by have ->: 3*q+q = 4*q by ring.
 seq 6 7: (#[/:11]pre /\
   I16u16_sb (5*q) r0{2} r0c{1} /\
   I16u16_sb (5*q) r1{2} r1c{1} /\
@@ -1618,7 +1695,7 @@ seq 6 7: (#[/:11]pre /\
   by rewrite /xx -iotaredE /= !z2u256E 1..2:// !C2RK /jzetas_exp /= -!inFqM_mod /q /= !Iu16_ub_of_int /q.
  have E: 7*q+q = 8*q by ring. 
  by rewrite /xx !E => {xx} -> |> *.
-seq 11 23: (i{2}=1 /\ #[/2,3]pre /\
+seq 11 23: (#[/:2]pre /\ i{2}=1 /\ 
   I16u16_ub (2*q) (P2R rp{2} 0) (P2C rp8{1} 0) /\
   I16u16_ub (2*q) (P2R rp{2} 1) (P2C rp8{1} 1) /\
   I16u16_ub (2*q) (P2R rp{2} 2) (P2C rp8{1} 2) /\
@@ -1657,12 +1734,10 @@ seq 11 23: (i{2}=1 /\ #[/2,3]pre /\
  move => |> *.
  rewrite (P2RS rp{2}) /= !PUR_i //= !P2R_i //= => |> *.
  by rewrite (P2CS rp{1}) /= !PUC_i //= !P2C_i //= => |> *.
+(* second iteration *)
 unroll {2} 1; rcondt {2} 1.
  by move=> &m; skip.
-rcondf {2} 63.
- by move=> &m; inline*; wp; skip.
-(* second iteration *)
-seq 10 11: (#[/:11]pre /\
+seq 10 8: (#[/:11]pre /\
   I16u16_sb (4*q) r0{2} r0l{1} /\
   I16u16_sb (4*q) r1{2} r1l{1} /\
   I16u16_sb (4*q) r2{2} r2l{1} /\
@@ -1671,6 +1746,7 @@ seq 10 11: (#[/:11]pre /\
   I16u16_sb (4*q) r5{2} r5l{1} /\
   I16u16_sb (4*q) r6{2} r6l{1} /\
   I16u16_sb (4*q) r7{2} r7l{1} ).
+ rcondf {2} 3; first by auto.
  wp; call (butterfly64x_eq (3*q)); wp; skip => &1 &2 |> *.
  have ->:  3 * q + q <= 32767 by rewrite /q.
  pose z0R := VPBROADCAST_8u32 _.
@@ -1777,6 +1853,7 @@ seq 6 7: (#[/:11]pre /\
   by rewrite /xx -iotaredE /= !z2u256E 1..2:// !C2RK /zetas_op /= -!inFqM_mod /q /= !Iu16_ub_of_int /q /=.
  have ->: 7*q+q = 8*q by ring. 
  by rewrite /xx => {xx} -> |> *.
+rcondf {2} 24; first by (move=> *; inline*; wp; auto).
 wp; ecall {2} (__red16x_ph r7u{1}).
 ecall {2} (__red16x_ph r3u{1}).
 ecall {2} (__red16x_ph r5u{1}).
@@ -1808,263 +1885,6 @@ move => |> *.
 by rewrite (P2RS rp{2}) (P2CS rp8{1}) /= !PUR_i //= !PUC_i //= -{2}iotaredE /= !P2R_i //= !P2C_i //=.
 qed.
 
-(* Alternative approach: 
-  obs: to investigates what causes the efficiency problems...
-equiv __ntt_level1t6_eq':
- NTT_AVX.__ntt_level1t6 ~ Jkem_avx2.M.__ntt_level1t6:
- I256u16_sb 3 rp{2} rp{1} ==> I256u16_ub 2 res{2} res{1}.
-proof.
-transitivity Tmp.__ntt_level1t6
- ( I256u16_sb 3 rp{2} rp{1} ==> I256u16_ub 2 res{2} res{1} )
- ( ={rp} ==> ={res} );
-  last by symmetry; conseq __ntt_level1t6_eq_.
-  move => &1 &2 *; exists arg{2}; smt().
- done.
-proc.
-unroll {2} 5; rcondt {2} 5.
- by move=> &m; wp;skip => /=.
-seq 45 66: (i{2} = 1 /\ zetasp{2}=zetas_op
-  /\ x16_spec q qx16{2} /\
-  I16u16_ub 2 (P2R rp{2} 0) (P2C rp8{1} 0) /\
-  I16u16_ub 2 (P2R rp{2} 1) (P2C rp8{1} 1) /\
-  I16u16_ub 2 (P2R rp{2} 2) (P2C rp8{1} 2) /\
-  I16u16_ub 2 (P2R rp{2} 3) (P2C rp8{1} 3) /\
-  I16u16_ub 2 (P2R rp{2} 4) (P2C rp8{1} 4) /\
-  I16u16_ub 2 (P2R rp{2} 5) (P2C rp8{1} 5) /\
-  I16u16_ub 2 (P2R rp{2} 6) (P2C rp8{1} 6) /\
-  I16u16_ub 2 (P2R rp{2} 7) (P2C rp8{1} 7) /\
-  I16u16_sb 3 (P2R rp{2} 8) (P2C rp{1} 8) /\
-  I16u16_sb 3 (P2R rp{2} 9) (P2C rp{1} 9) /\
-  I16u16_sb 3 (P2R rp{2} 10) (P2C rp{1} 10) /\
-  I16u16_sb 3 (P2R rp{2} 11) (P2C rp{1} 11) /\
-  I16u16_sb 3 (P2R rp{2} 12) (P2C rp{1} 12) /\
-  I16u16_sb 3 (P2R rp{2} 13) (P2C rp{1} 13) /\
-  I16u16_sb 3 (P2R rp{2} 14) (P2C rp{1} 14) /\
-  I16u16_sb 3 (P2R rp{2} 15) (P2C rp{1} 15) ).
- (* first iteration (first 128 coefs) *)
- wp.
- ecall {2} (__red16x_ph r7j{1}).
- ecall {2} (__red16x_ph r3j{1}).
- ecall {2} (__red16x_ph r5j{1}).
- ecall {2} (__red16x_ph r1j{1}).
- ecall {2} (__red16x_ph r6j{1}).
- ecall {2} (__red16x_ph r2j{1}).
- ecall {2} (__red16x_ph r4j{1}).
- ecall {2} (__red16x_ph r0j{1}).
- wp; call (butterfly64x_eq 8).
- wp; call (butterfly64x_eq 7).
- ecall {2} (__shuffle1_ph 7 r3g{1} r7g{1}).
- ecall {2} (__shuffle1_ph 7 r2g{1} r6g{1}).
- ecall {2} (__shuffle1_ph 7 r1g{1} r5g{1}).
- ecall {2} (__shuffle1_ph 7 r0g{1} r4g{1}).
- wp; call (butterfly64x_eq 6); simplify.
- ecall {2} (__shuffle2_ph 6 r6e{1} r7e{1}).
- ecall {2} (__shuffle2_ph 6 r4e{1} r5e{1}).
- ecall {2} (__shuffle2_ph 6 r2e{1} r3e{1}).
- ecall {2} (__shuffle2_ph 6 r0e{1} r1e{1}).
- wp; call (butterfly64x_eq 5); simplify.
- ecall {2} (__shuffle4_ph 5 r5c{1} r7c{1}).
- ecall {2} (__shuffle4_ph 5 r1c{1} r3c{1}).
- ecall {2} (__shuffle4_ph 5 r4c{1} r6c{1}).
- ecall {2} (__shuffle4_ph 5 r0c{1} r2c{1}).
- wp; call (butterfly64x_eq 4); simplify.
- ecall {2} (__shuffle8_ph 4 r3a{1} r7a{1}).
- ecall {2} (__shuffle8_ph 4 r2a{1} r6a{1}).
- ecall {2} (__shuffle8_ph 4 r1a{1} r5a{1}).
- ecall {2} (__shuffle8_ph 4 r0a{1} r4a{1}).
- wp; call (butterfly64x_eq 3); simplify.
-time wp; skip => &1 &2 Hpre (*zetas*) qx16 z0R z1R z1L.
- have ->: 3 * q + q <= 32767 by smt().
- have ->: qinv16u16M z0R z1R.
-  by rewrite /z0R /z1R /zR !z2u32E //= /VPBROADCAST_8u32 /qinv16u16M -iotaredE /=.
- have ->: x16_spec q qx16.
-  by rewrite x16_spec_C2R /q /=.
- have ->: I16u16M_ub 1 z1R z1L.
-  by rewrite /z1L /z1R /zR !z2u32E //= /VPBROADCAST_8u32 /R2C -iotaredE /= -inFqM_mod /q !Iu16_ub_of_int /#.
- move: Hpre; rewrite -{2}iotaredE /= => |> *.
- have ->: 4 * q + q <= 32767 by smt().
- have ->: qinv16u16M (z2u256 zetas_op 8) (z2u256 zetas_op 24).
-  rewrite !z2u256E 1..2:// /qinv16u16M -iotaredE.
-  by rewrite /= !C2RK !initiE.
- pose xx := List.all _ _.
- have: xx.
-  by rewrite /xx -iotaredE /= !z2u256E // !C2RK /zetas_op /= -!inFqM_mod /q /= !Iu16_ub_of_int /q.
- rewrite /xx => {xx} -> |> *.
- have ->: 5 * q + q <= 32767 by smt().
- have ->: qinv16u16M (z2u256 zetas_op 40) (z2u256 zetas_op 56).
-  rewrite !z2u256E 1..2:// /qinv16u16M -iotaredE.
-  by rewrite /= !C2RK !initiE.
- pose xx := List.all _ _.
- have: xx.
-  by rewrite /xx -iotaredE /= !z2u256E // !C2RK /zetas_op /= -!inFqM_mod /q /= !Iu16_ub_of_int /q.
- rewrite /xx => {xx} -> |> *.
- have ->: 6 * q + q <= 32767 by smt().
- have ->: qinv16u16M (z2u256 zetas_op 72) (z2u256 zetas_op 88).
-  by rewrite !z2u256E 1..2:// /qinv16u16M -iotaredE           /= !C2RK !initiE /=.
- pose xx := List.all _ _.
- have: xx.
-  by rewrite /xx -iotaredE /= !z2u256E // !C2RK /zetas_op /= -!inFqM_mod /q /= !Iu16_ub_of_int /q.
- rewrite /xx => {xx} -> |> *.
- have ->: 7 * q + q <= 32767 by smt().
- have ->: qinv16u16M (z2u256 zetas_op 104) (z2u256 zetas_op 120).
-  by rewrite !z2u256E 1..2:// /qinv16u16M -iotaredE           /= !C2RK !initiE /=.
- pose xx := List.all _ _.
- have: xx.
-  by rewrite /xx -iotaredE /= !z2u256E // !C2RK /zetas_op /= -!inFqM_mod /q /= !Iu16_ub_of_int /q.
- rewrite /xx => {xx} -> |> *.
- have ->: 8 * q + q <= 32767 by smt().
- have ->: qinv16u16M (z2u256 zetas_op 136) (z2u256 zetas_op 152).
-  by rewrite !z2u256E 1..2:// /qinv16u16M -iotaredE           /= !C2RK !initiE /=.
- have ->: qinv16u16M (z2u256 zetas_op 168) (z2u256 zetas_op 184).
-  by rewrite !z2u256E 1..2:// /qinv16u16M -iotaredE           /= !C2RK !initiE /=.
- pose xxa := List.all _ _.
- have ->: xxa.
-  by rewrite /xxa -iotaredE /= !z2u256E // !C2RK /zetas_op /= -!inFqM_mod /q /= !Iu16_ub_of_int /q.
- pose xxb := List.all _ _.
- have ->: xxb.
-  by rewrite /xxb -iotaredE /= !z2u256E // !C2RK /zetas_op /= -!inFqM_mod /q /= !Iu16_ub_of_int /q.
- rewrite /xxb => {xxa xxb} |> *.
- have Hvx16: x16_spec 20159 (C2R vx16_op).
-  by rewrite x16_spec_C2R /q /=.
- move => |> *.
- rewrite (P2RS rp{2}) /= !PUR_i //= !P2R_i //= => |> *.
- by rewrite (P2CS rp{1}) /= !PUC_i //= !P2C_i //= => |> *.
-unroll {2} 1; rcondt {2} 1.
- by move=> &m; skip.
-rcondf {2} 63.
- by move=> &m; inline*; wp; skip.
-(* second iteration *)
-wp.
-ecall {2} (__red16x_ph r7u{1}).
-ecall {2} (__red16x_ph r3u{1}).
-ecall {2} (__red16x_ph r5u{1}).
-ecall {2} (__red16x_ph r1u{1}).
-ecall {2} (__red16x_ph r6u{1}).
-ecall {2} (__red16x_ph r2u{1}).
-ecall {2} (__red16x_ph r4u{1}).
-ecall {2} (__red16x_ph r0u{1}).
-wp; call (butterfly64x_eq 8).
-wp; call (butterfly64x_eq 7).
-ecall {2} (__shuffle1_ph 7 r3r{1} r7r{1}).
-ecall {2} (__shuffle1_ph 7 r2r{1} r6r{1}).
-ecall {2} (__shuffle1_ph 7 r1r{1} r5r{1}).
-ecall {2} (__shuffle1_ph 7 r0r{1} r4r{1}).
-wp; call (butterfly64x_eq 6); simplify.
-ecall {2} (__shuffle2_ph 6 r6p{1} r7p{1}).
-ecall {2} (__shuffle2_ph 6 r4p{1} r5p{1}).
-ecall {2} (__shuffle2_ph 6 r2p{1} r3p{1}).
-ecall {2} (__shuffle2_ph 6 r0p{1} r1p{1}).
-wp; call (butterfly64x_eq 5); simplify.
-ecall {2} (__shuffle4_ph 5 r5n{1} r7n{1}).
-ecall {2} (__shuffle4_ph 5 r1n{1} r3n{1}).
-ecall {2} (__shuffle4_ph 5 r4n{1} r6n{1}).
-ecall {2} (__shuffle4_ph 5 r0n{1} r2n{1}).
-wp; call (butterfly64x_eq 4); simplify.
-ecall {2} (__shuffle8_ph 4 r3l{1} r7l{1}).
-ecall {2} (__shuffle8_ph 4 r2l{1} r6l{1}).
-ecall {2} (__shuffle8_ph 4 r1l{1} r5l{1}).
-ecall {2} (__shuffle8_ph 4 r0l{1} r4l{1}).
-wp; call (butterfly64x_eq 3); simplify.
-wp; skip => &1 &2 [-> [Ezetas |>]] *.
-pose z0R := VPBROADCAST_8u32 _.
-pose z1R := VPBROADCAST_8u32 _.
-pose z1L := Array16.init _.
-have ->: 3 * q + q <= 32767 by smt().
-have ->: qinv16u16M z0R z1R.
- by rewrite /z0R /z1R !z2u32E //= /VPBROADCAST_8u32 /qinv16u16M -iotaredE /R2C !Ezetas /=.
-have ->: I16u16M_ub 1 z1R z1L.
- by rewrite /z1L /z1R !z2u32E //= /VPBROADCAST_8u32 /R2C -iotaredE /= -inFqM_mod /q /= Ezetas !initiE //= !Iu16_ub_of_int /q /=.
-move => |> *.
-clear z0R z1R z1L.
-pose z0R := z2u256 _ _.
-pose z1R := z2u256 _ _.
-pose z1L := Array16.of_list _ _.
-have ->: 4 * q + q <= 32767 by smt().
-have ->: qinv16u16M z0R z1R.
- rewrite /z0R /z1R !z2u256E 1..2:// /qinv16u16M -iotaredE.
- by rewrite /= !C2RK !Ezetas !initiE //=.
-pose xx := List.all _ _.
-have: xx.
- by rewrite /xx /z1R /z1L -iotaredE /= !z2u256E // !C2RK Ezetas /= -!inFqM_mod /q /= !Iu16_ub_of_int /q.
-rewrite /xx => {xx} -> |> *.
-clear z0R z1R z1L.
-pose z0R := z2u256 _ _.
-pose z1R := z2u256 _ _.
-pose z1L := Array16.of_list _ _.
-have ->: 5 * q + q <= 32767 by smt().
-have ->: qinv16u16M z0R z1R.
- rewrite /z0R /z1R !z2u256E 1..2:// /qinv16u16M -iotaredE.
- by rewrite /= !C2RK !Ezetas !initiE //=.
-pose xx := List.all _ _.
-have: xx.
- by rewrite /xx /z1R /z1L -iotaredE /= !z2u256E // !C2RK Ezetas /= -!inFqM_mod /q /= !Iu16_ub_of_int /q.
-rewrite /xx => {xx} -> |> *.
-clear z0R z1R z1L.
-pose z0R := z2u256 _ _.
-pose z1R := z2u256 _ _.
-pose z1L := Array16.of_list _ _.
-have ->: 6 * q + q <= 32767 by smt().
-have ->: qinv16u16M z0R z1R.
- rewrite /z0R /z1R !z2u256E 1..2:// /qinv16u16M -iotaredE.
- by rewrite /= !C2RK !Ezetas !initiE //=.
-pose xx := List.all _ _.
-have: xx.
- by rewrite /xx /z1R /z1L -iotaredE /= !z2u256E // !C2RK Ezetas /= -!inFqM_mod /q /= !Iu16_ub_of_int /q.
-rewrite /xx => {xx} -> |> *.
-clear z0R z1R z1L.
-pose z0R := z2u256 _ _.
-pose z1R := z2u256 _ _.
-pose z1L := Array16.of_list _ _.
-have ->: 7 * q + q <= 32767 by smt().
-have ->: qinv16u16M z0R z1R.
- rewrite /z0R /z1R !z2u256E 1..2:// /qinv16u16M -iotaredE.
- by rewrite /= !C2RK !Ezetas !initiE //=.
-pose xx := List.all _ _.
-have: xx.
- by rewrite /xx /z1R /z1L -iotaredE /= !z2u256E // !C2RK Ezetas /= -!inFqM_mod /q /= !Iu16_ub_of_int /q.
-rewrite /xx => {xx} -> |> *.
-clear z0R z1R z1L.
-pose z0Ra := z2u256 _ _.
-pose z1Ra := z2u256 _ _.
-pose z1La := Array16.of_list _ _.
-pose z0Rb := z2u256 _ _.
-pose z1Rb := z2u256 _ _.
-pose z1Lb := Array16.of_list _ _.
-have ->: 8 * q + q <= 32767 by smt().
-have ->: qinv16u16M z0Ra z1Ra.
- rewrite /z0Ra /z1Ra !z2u256E 1..2:// /qinv16u16M -iotaredE.
- by rewrite /= !C2RK !Ezetas !initiE //=.
-have ->: qinv16u16M z0Rb z1Rb.
- rewrite /z0Rb /z1Rb !z2u256E 1..2:// /qinv16u16M -iotaredE.
- by rewrite /= !C2RK !Ezetas !initiE //=.
-pose xxa := List.all _ _.
-have: xxa.
- by rewrite /xxa /z1Ra /z1La -iotaredE /= !z2u256E // !C2RK Ezetas /= -!inFqM_mod /q /= !Iu16_ub_of_int /q.
-rewrite /xxa => {xxa} ->; pose xxb := List.all _ _.
-have: xxb.
- by rewrite /xxb /z1Rb /z1Lb -iotaredE /= !z2u256E // !C2RK Ezetas /= -!inFqM_mod /q /= !Iu16_ub_of_int /q.
-rewrite /xxb => {xxb} -> |> *.
-clear z0Ra z1Ra z1La z0Rb z1Rb z1Lb.
-have Hvx16: x16_spec 20159 (C2R vx16_op).
- by rewrite x16_spec_C2R /q /=.
-move => |> *.
-by rewrite (P2RS rp{2}) (P2CS rp8{1}) /= !PUR_i //= !PUC_i //= -{2}iotaredE /= !P2R_i //= !P2C_i //=.
-qed.
-*)
-
-equiv _poly_ntt_eq:
- NTT_AVX.ntt ~Jkem_avx2.M._poly_ntt:
- r{1}=lift_array256 rp{2} /\ signed_bound_cxq rp{2} 0 256 2 ==>
- res{1}=lift_array256 res{2} /\
- pos_bound256_cxq res{2} 0 256 2.
-proof.
-proc.
-conseq (_: I256u16_sb (2*q) rp{2} r{1} ==> I256u16_ub (2*q) rp{2} rp6{1} ).
-  by move=> &1 &2; rewrite I256u16_sbE.
- by move => &1 &2 /= ???; rewrite -I256u16_ubE.
-call __ntt_level1t6_eq.
-by call __ntt_level0_eq.
-qed.
 
 lemma invntt_butterfly16xE (n1 n2:int) xl xr z rxl rxr rzM rzMqinv rq16x:
  n1+n2 <= W16.max_sint =>
@@ -2105,7 +1925,7 @@ equiv invntt_butterfly64x_eq c0 c1 c2 c3 c4 c5 c6 c7:
  ~ Jkem_avx2.M.__invntt___butterfly64x :
  MAX (MAX (c0+c4) (c1+c5))%Int
      (MAX (c2+c6) (c3+c7))%Int
-  *q <= W16.max_sint /\
+  <= W16.max_sint /\
  I16u16_sb c0 rl0{2} rl0t{1} /\
  I16u16_sb c1 rl1{2} rl1t{1} /\
  I16u16_sb c2 rl2{2} rl2t{1} /\
@@ -2152,22 +1972,102 @@ by apply (invntt_butterfly16xE c); smt().
 *).
 qed.
 
+abbrev mul16x1 (x: Fq Array16.t) y: Fq Array16.t =
+ Array16.init (fun i => x.[i]*y).
+abbrev mul16x16 (x y: Fq Array16.t): Fq Array16.t =
+ Array16.init (fun i => x.[i]*y.[i]).
 
-(*
-equiv __invntt_level0t5_eq:
- NTT_AVX.__invntt_level0t5 ~ Jkem_avx2.M.__invntt_levels0t5:
- I256u16_sb 2 rp{2} rp{1} ==> I256u16_sb 3 res{2} res{1}.
+lemma P2C_mul16x1 (l: Fq Array16.t list) k x:
+  size l = 16 =>
+  0 <= k < 16 =>
+  P2C (Array256.init (fun i=>(CS2P l).[i]*x)) k
+  = mul16x1 (nth witness l k) x.
 proof.
-transitivity Tmp.__invntt_levels0t5ALT
- ( I256u16_sb (2*q) rp{2} rp{1} ==> I256u16_sb 3 res{2} res{1} )
- ( ={rp} ==> ={res} );
-  last by symmetry; conseq __invntt_levels0t5_eq_.
-  move => &1 &2 *; exists arg{2}; smt().
- done.
+move=> Hsize Hk.
+have ->: Array256.init (fun i => (CS2P l).[i]*x)
+         = CS2P (List.map (Array16.map (fun y=>y*x)) l).
+ rewrite tP => i Hi /=.
+ rewrite initiE 1:/# /=.
+ rewrite /CS2P /punchunk !initiE //= !get_of_list 1..2:/#.
+ by rewrite (nth_map witness) 1:/# mapE initiE 1:/# /=. 
+rewrite P2C_i 1://.
+ by rewrite size_map.
+by rewrite (nth_map witness) 1..2://; smt().
+qed.
+
+equiv invntt_butterfly64x_eq_last x c0 c1 c2 c3 c4 c5 c6 c7:
+ NTT_AVX.__invntt___butterfly64x
+ ~ Jkem_avx2.M.__invntt___butterfly64x :
+ MAX (MAX (c0+c4) (c1+c5))%Int
+     (MAX (c2+c6) (c3+c7))%Int
+  <= W16.max_sint /\
+ I16u16_sb c0 rl0{2} rl0t{1} /\
+ I16u16_sb c1 rl1{2} rl1t{1} /\
+ I16u16_sb c2 rl2{2} rl2t{1} /\
+ I16u16_sb c3 rl3{2} rl3t{1} /\
+ I16u16_sb c4 rh0{2} rh0t{1} /\
+ I16u16_sb c5 rh1{2} rh1t{1} /\
+ I16u16_sb c6 rh2{2} rh2t{1} /\
+ I16u16_sb c7 rh3{2} rh3t{1} /\
+ qinv16u16M zl0{2} zh0{2} /\
+ qinv16u16M zl1{2} zh1{2} /\
+ I16u16M_ub q zh0{2} (mul16x1 z0{1} (x*inFq 65536)) /\
+ I16u16M_ub q zh1{2} (mul16x1 z1{1} (x*inFq 65536)) /\
+ x16_spec q qx16{2}
+ ==>
+ I16u16_sb (c0+c4) res{2}.`1 res{1}.`1 /\
+ I16u16_sb (c1+c5) res{2}.`2 res{1}.`2 /\
+ I16u16_sb (c2+c6) res{2}.`3 res{1}.`3 /\
+ I16u16_sb (c3+c7) res{2}.`4 res{1}.`4 /\
+ I16u16_sb q res{2}.`5 (mul16x1 res{1}.`5 x) /\
+ I16u16_sb q res{2}.`6 (mul16x1 res{1}.`6 x) /\
+ I16u16_sb q res{2}.`7 (mul16x1 res{1}.`7 x) /\
+ I16u16_sb q res{2}.`8 (mul16x1 res{1}.`8 x).
+admitted.
+
+
+phoare fqmulprecomp16x_ph n _a _b:
+ [ Jkem_avx2.M.__fqmulprecomp16x :
+   qinv16u16M al ah =>
+   I16u16M_ub q ah _a =>
+   I16u16_sb n b _b
+   ==> I16u16_sb q res (mul16x16 _a _b) ] = 1%r.
+admitted.
+
+abbrev Iu16 y x = x = inFqW16 y.
+abbrev I16u16 y (x:Fq Array16.t) = all (fun k=>Iu16 (R2C y).[k] x.[k]) (iota_ 0 16).
+
+phoare red16x_aux _n _r:
+ [ Jkem_avx2.M.__red16x :
+   x16_spec q qx16 =>
+   x16_spec 20159 vx16 =>
+   I16u16_sb _n r _r
+   ==> I16u16_sb (2*q) res _r ] = 1%r.
+admitted.
+
+phoare fq_mulprecomp16x_aux _n _r:
+ [ Jkem_avx2.M.__fqmulprecomp16x :
+   x16_spec q qx16 =>
+   x16_spec 1441 ah =>
+   qinv16u16M al ah =>
+   I16u16_sb _n b _r
+   ==> I16u16_sb q res (mul16x1 _r (inFq 3303)) ] = 1%r.
+admitted.
+
+equiv _poly_invntt_eq:
+ NTT_AVX.invntt ~ Jkem_avx2.M._poly_invntt:
+ rp{1}=lift_array256 rp{2} /\ signed_bound_cxq rp{2} 0 256 2 ==>
+ res{1}=lift_array256 res{2} /\
+ signed_bound_cxq res{2} 0 256 1.
+proof.
+transitivity Tmp._invntt
+ ( I256u16_sb (2*q) rp{2} rp{1} ==> I256u16_sb q res{2} res{1} )
+ ( ={rp} ==> ={res} ); last by symmetry; conseq __invntt_eq_.
+  by move=> |> &2 H; exists arg{2}; rewrite I256u16_sbE. 
+ by move => &1 &m &2 /= ??; rewrite -I256u16_sbE /#.
 proc.
-unroll {2} 6; rcondt {2} 6.
- by move=> &m; wp;skip.
-seq 12 20: (i{2} = 0 /\ zetasp{2}=zetas_op  /\ x16_spec q qx16{2} /\ x16_spec 20159 vx16{2} /\
+unroll{2} 4; rcondt{2} 4; first by auto.
+seq 11 16: (x16_spec q qx16{2} /\ zetasp{2}=zetas_inv_op  /\ i{2}=0 /\
   I16u16_sb (2*q) (P2R rp{2} 8) (P2C rp{1} 8) /\
   I16u16_sb (2*q) (P2R rp{2} 9) (P2C rp{1} 9) /\
   I16u16_sb (2*q) (P2R rp{2} 10) (P2C rp{1} 10) /\
@@ -2178,329 +2078,457 @@ seq 12 20: (i{2} = 0 /\ zetasp{2}=zetas_op  /\ x16_spec q qx16{2} /\ x16_spec 20
   I16u16_sb (2*q) (P2R rp{2} 15) (P2C rp{1} 15) /\
   I16u16_sb (4*q) r0{2} r0a{1} /\
   I16u16_sb (4*q) r1{2} r1a{1} /\
-  I16u16_sb 1 r2{2} r2a{1} /\
-  I16u16_sb 1 r3{2} r3a{1} /\
-  I16u16_sb 4 r4{2} r4a{1} /\
-  I16u16_sb 4 r5{2} r5a{1} /\
-  I16u16_sb 1 r6{2} r6a{1} /\
-  I16u16_sb 1 r7{2} r7a{1} ).
- admit(*
- wp; call (butterfly64x_eq 3); wp; skip => &1 &2 Hpre qx16 z0R z1R |>.
- have ->:  3 * q + q <= 32767 by rewrite /q.
+  I16u16_sb (1*q) r2{2} r2a{1} /\
+  I16u16_sb (1*q) r3{2} r3a{1} /\
+  I16u16_sb (4*q) r4{2} r4a{1} /\
+  I16u16_sb (4*q) r5{2} r5a{1} /\
+  I16u16_sb (1*q) r6{2} r6a{1} /\
+  I16u16_sb (1*q) r7{2} r7a{1}).
+ call (invntt_butterfly64x_eq (2*q) (2*q) (2*q) (2*q) (2*q) (2*q) (2*q) (2*q)).
+ wp; skip => &1 &2.
+ rewrite -{2}iotaredE /= => [#] |> *.
+ pose z0R := z2u256 _ _.
+ pose z1R := z2u256 _ _.
+ pose z2R := z2u256 _ _.
+ pose z3R := z2u256 _ _.
+ pose z1L := Array16.of_list _ _.
+ pose z3L := Array16.of_list _ _.
+ have ->: 2*q + 2*q <= 32767 by smt().
  have ->: qinv16u16M z0R z1R.
-  by rewrite /z0R /z1R /zR !z2u32E 1..2://= /VPBROADCAST_8u32 /qinv16u16M -iotaredE /=.
- have ->: x16_spec q qx16.
+  rewrite /z0R /z1R !z2u256E 1..2:// /qinv16u16M -iotaredE.
+  by rewrite /= !C2RK /zetas_inv_op !initiE //=.
+ have ->: qinv16u16M z2R z3R.
+  rewrite /z2R /z3R !z2u256E 1..2:// /qinv16u16M -iotaredE.
+  by rewrite /= !C2RK /zetas_inv_op !initiE //=.
+ pose xx := List.all _ _.
+ have ->: xx.
+  by rewrite /xx /z1R /z1L -iotaredE /= !z2u256E // !C2RK /zetas_inv_op /= -!inFqM_mod /q /= !Iu16_ub_of_int /q.
+ clear xx; pose xx := List.all _ _.
+ have ->: xx.
+  by rewrite /xx /z3R /z3L -iotaredE /= !z2u256E // !C2RK /zetas_inv_op /= -!inFqM_mod /q /= !Iu16_ub_of_int /q.
+ have ->: x16_spec q (C2R qx16_op).
   by rewrite x16_spec_C2R /q /=.
- pose z1L:= Array16.init _.
- have ->: I16u16M_ub 1 z1R z1L.
-  by rewrite /z1L /z1R /zR !z2u32E 1..2://= /VPBROADCAST_8u32 /R2C -iotaredE /= -inFqM_mod /q !Iu16_ub_of_int /#. 
- by move: Hpre; rewrite -{2}iotaredE /= => |> *.*).
-seq 6 9: (#[/:12]pre /\
-  I16u16_sb 2 r0{2} r0c{1} /\ (* 8 => 2 *)
-  I16u16_sb 2 r1{2} r1c{1} /\ (* 8 => 2 *)
-  I16u16_sb 2 r2{2} r2c{1} /\
-  I16u16_sb 2 r3{2} r3c{1} /\
-  I16u16_sb 1 r4{2} r4c{1} /\
-  I16u16_sb 1 r5{2} r5c{1} /\
-  I16u16_sb 1 r6{2} r6c{1} /\
-  I16u16_sb 1 r7{2} r7c{1} ).
-admit(*
- wp; call (butterfly64x_eq 4).
- ecall {2} (__shuffle8_ph 4 r3a{1} r7a{1}).
- ecall {2} (__shuffle8_ph 4 r2a{1} r6a{1}).
- ecall {2} (__shuffle8_ph 4 r1a{1} r5a{1}).
- ecall {2} (__shuffle8_ph 4 r0a{1} r4a{1}).
- wp; skip => &1 &2 |> /= *.
- have ->:  4 * q + q <= 32767 by rewrite /q.
- have ->: qinv16u16M (z2u256 zetas_op 8) (z2u256 zetas_op 24).
-  rewrite !z2u256E 1..2:// /qinv16u16M -iotaredE /=.
-  by rewrite /= !C2RK !initiE 1..32:// /jzetas_exp /=.
+ clear xx z0R z1R z2R z3R z1L z3L => |>.
+ by have ->: 2*q+2*q = 4*q by ring.
+seq 2 4: (#[/:11]pre /\ x16_spec 20159 vx16{2} /\
+  I16u16_sb (8*q) r0{2} r0b{1} /\ (* 8 => 2 *)
+  I16u16_sb (8*q) r1{2} r1b{1} /\ (* 8 => 2 *)
+  I16u16_sb (2*q) r2{2} r2b{1} /\
+  I16u16_sb (2*q) r3{2} r3b{1} /\
+  I16u16_sb (1*q) r4{2} r4b{1} /\
+  I16u16_sb (1*q) r5{2} r5b{1} /\
+  I16u16_sb (1*q) r6{2} r6b{1} /\
+  I16u16_sb (1*q) r7{2} r7b{1} ).
+ call (invntt_butterfly64x_eq (4*q) (4*q) (1*q) (1*q) (4*q) (4*q) (1*q) (1*q)).
+ wp; skip => |> &1 &2 *.
+ pose z0R := z2u256 _ _.
+ pose z1R := z2u256 _ _.
+ pose z1L := Array16.of_list _ _.
+ have ->: MAX (4 * q + 4 * q) (q + q) <= 32767 by smt().
+ have ->: qinv16u16M z0R z1R.
+  rewrite /z0R /z1R !z2u256E 1..2:// /qinv16u16M -iotaredE.
+  by rewrite /= !C2RK /zetas_inv_op !initiE //=.
  pose xx := List.all _ _.
- have: xx.
-  by rewrite /xx -iotaredE /= !z2u256E 1..2:// !C2RK /jzetas_exp /= -!inFqM_mod /q /= !Iu16_ub_of_int /q.
- by rewrite /xx => {xx} -> |> *.*).
-seq 6 7: (#[/:12]pre /\
-  I16u16_sb 4 r0{2} r0e{1} /\
-  I16u16_sb 1 r1{2} r1e{1} /\
-  I16u16_sb 4 r2{2} r2e{1} /\
-  I16u16_sb 1 r3{2} r3e{1} /\
-  I16u16_sb 2 r4{2} r4e{1} /\
-  I16u16_sb 1 r5{2} r5e{1} /\
-  I16u16_sb 2 r6{2} r6e{1} /\
-  I16u16_sb 1 r7{2} r7e{1} ).
-admit(*
- wp; call (butterfly64x_eq 5).
- ecall {2} (__shuffle4_ph 5 r5c{1} r7c{1}).
- ecall {2} (__shuffle4_ph 5 r1c{1} r3c{1}).
- ecall {2} (__shuffle4_ph 5 r4c{1} r6c{1}).
- ecall {2} (__shuffle4_ph 5 r0c{1} r2c{1}).
- wp; skip => &1 &2 |> *.
- have ->:  5 * q + q <= 32767 by rewrite /q.
- have ->: qinv16u16M (z2u256 jzetas_exp 40) (z2u256 jzetas_exp 56).
-  rewrite !z2u256E 1..2:// /qinv16u16M -iotaredE.
-  by rewrite /= !C2RK !initiE 1..32:// /jzetas_exp /=.
- pose xx := List.all _ _.
- have: xx.
-  by rewrite /xx -iotaredE /= !z2u256E 1..2:// !C2RK /jzetas_exp /= -!inFqM_mod /q /= !Iu16_ub_of_int /q /=.
- by rewrite /xx => {xx} -> |> *.
-*).
-seq 6 8: (#[/:12]pre /\
-  I16u16_sb 2 r0{2} r0g{1} /\ (* 8 => 2 *)
-  I16u16_sb 2 r1{2} r1g{1} /\
-  I16u16_sb 1 r2{2} r2g{1} /\
-  I16u16_sb 1 r3{2} r3g{1} /\
-  I16u16_sb 4 r4{2} r4g{1} /\
-  I16u16_sb 2 r5{2} r5g{1} /\
-  I16u16_sb 1 r6{2} r6g{1} /\
-  I16u16_sb 1 r7{2} r7g{1} ).
-admit (*
- wp; call (butterfly64x_eq 6).
- ecall {2} (__shuffle2_ph 6 r6e{1} r7e{1}).
- ecall {2} (__shuffle2_ph 6 r4e{1} r5e{1}).
- ecall {2} (__shuffle2_ph 6 r2e{1} r3e{1}).
- ecall {2} (__shuffle2_ph 6 r0e{1} r1e{1}).
- wp; skip => &1 &2 |> *.
- have ->:  6 * q + q <= 32767 by rewrite /q.
- have ->: qinv16u16M (z2u256 jzetas_exp 72) (z2u256 jzetas_exp 88).
-  rewrite !z2u256E 1..2:// /qinv16u16M -iotaredE.
-  by rewrite /= !C2RK !initiE 1..32:// /jzetas_exp /=.
- pose xx := List.all _ _.
- have: xx.
-  by rewrite /xx -iotaredE /= !z2u256E 1..2:// !C2RK /jzetas_exp /= -!inFqM_mod /q /= !Iu16_ub_of_int /q /=.
- by rewrite /xx => {xx} -> |> *.
-*).
-seq 6 8: (#[/:12]pre /\
-  I16u16_sb 2 r0{2} r0i{1} /\ (* 8 => 2 *)
-  I16u16_sb 4 r1{2} r1i{1} /\
-  I16u16_sb 2 r2{2} r2i{1} /\
-  I16u16_sb 2 r3{2} r3i{1} /\
-  I16u16_sb 1 r4{2} r4i{1} /\
-  I16u16_sb 1 r5{2} r5i{1} /\
-  I16u16_sb 1 r6{2} r6i{1} /\
-  I16u16_sb 1 r7{2} r7i{1} ).
-admit(*
- wp; call (butterfly64x_eq 7).
- ecall {2} (__shuffle1_ph 7 r3g{1} r7g{1}).
- ecall {2} (__shuffle1_ph 7 r2g{1} r6g{1}).
- ecall {2} (__shuffle1_ph 7 r1g{1} r5g{1}).
- ecall {2} (__shuffle1_ph 7 r0g{1} r4g{1}).
- wp; skip => &1 &2 |> *.
- have ->:  7 * q + q <= 32767 by rewrite /q.
- have ->: qinv16u16M (z2u256 jzetas_exp 104) (z2u256 jzetas_exp 120).
-  rewrite !z2u256E 1..2:// /qinv16u16M -iotaredE.
-  by rewrite /= !C2RK !initiE 1..32:// /jzetas_exp /=.
- pose xx := List.all _ _.
- have: xx.
-  by rewrite /xx -iotaredE /= !z2u256E 1..2:// !C2RK /jzetas_exp /= -!inFqM_mod /q /= !Iu16_ub_of_int /q.
- by rewrite /xx => {xx} -> |> *.
-*).
-seq 11 23: (i{2}=1 /\ #[/2,3]pre /\
-  I16u16_ub 2 (P2R rp{2} 0) (P2C rp8{1} 0) /\
-  I16u16_ub 2 (P2R rp{2} 1) (P2C rp8{1} 1) /\
-  I16u16_ub 2 (P2R rp{2} 2) (P2C rp8{1} 2) /\
-  I16u16_ub 2 (P2R rp{2} 3) (P2C rp8{1} 3) /\
-  I16u16_ub 2 (P2R rp{2} 4) (P2C rp8{1} 4) /\
-  I16u16_ub 2 (P2R rp{2} 5) (P2C rp8{1} 5) /\
-  I16u16_ub 2 (P2R rp{2} 6) (P2C rp8{1} 6) /\
-  I16u16_ub 2 (P2R rp{2} 7) (P2C rp8{1} 7) /\ #[/4:11]pre).
- wp; ecall {2} (__red16x_ph r7j{1}).
- ecall {2} (__red16x_ph r3j{1}).
- ecall {2} (__red16x_ph r5j{1}).
- ecall {2} (__red16x_ph r1j{1}).
- ecall {2} (__red16x_ph r6j{1}).
- ecall {2} (__red16x_ph r2j{1}).
- ecall {2} (__red16x_ph r4j{1}).
- ecall {2} (__red16x_ph r0j{1}).
- wp; call (butterfly64x_eq 8).
- wp; skip => &1 &2 |> *.
- have ->:  8 * q + q <= 32767 by rewrite /q /=.
- have ->: qinv16u16M (z2u256 jzetas_exp 136) (z2u256 jzetas_exp 152).
-  rewrite !z2u256E 1..2:// /qinv16u16M -iotaredE.
-  by rewrite /= !C2RK !initiE 1..32:// /jzetas_exp /=.
- have ->: qinv16u16M (z2u256 jzetas_exp 168) (z2u256 jzetas_exp 184).
-  rewrite !z2u256E 1..2:// /qinv16u16M -iotaredE.
-  by rewrite /= !C2RK !initiE 1..32:// /jzetas_exp /=.
- pose xx := List.all _ _.
- have: xx.
-  by rewrite /xx -iotaredE /= !z2u256E 1..2:// !C2RK /jzetas_exp /= -!inFqM_mod /q /= !Iu16_ub_of_int /q /=.
- rewrite /xx => {xx} ->; pose xx := List.all _ _.
- have: xx.
-  by rewrite /xx -iotaredE /= !z2u256E 1..2:// !C2RK /jzetas_exp /= -!inFqM_mod /q /= !Iu16_ub_of_int /q /=.
- rewrite /xx => {xx} -> |> *.
- have Hvx16: x16_spec 20159 (C2R vx16_op).
-  by rewrite x16_spec_C2R /q /=.
+ have ->: xx.
+  by rewrite /xx /z1R /z1L -iotaredE /= !z2u256E // !C2RK /zetas_inv_op /= -!inFqM_mod /q /= !Iu16_ub_of_int /q.
  move => |> *.
- rewrite (P2RS rp{2}) /= !PUR_i //= !P2R_i //= => |> *.
- by rewrite (P2CS rp{1}) /= !PUC_i //= !P2C_i //= => |> *.
-unroll {2} 1; rcondt {2} 1.
- by move=> &m; skip.
-rcondf {2} 63.
- by move=> &m; inline*; wp; skip.
-(* second iteration *)
-seq 10 11: (#[/:11]pre /\
-  I16u16_sb 4 r0{2} r0l{1} /\
-  I16u16_sb 4 r1{2} r1l{1} /\
-  I16u16_sb 4 r2{2} r2l{1} /\
-  I16u16_sb 4 r3{2} r3l{1} /\
-  I16u16_sb 4 r4{2} r4l{1} /\
-  I16u16_sb 4 r5{2} r5l{1} /\
-  I16u16_sb 4 r6{2} r6l{1} /\
-  I16u16_sb 4 r7{2} r7l{1} ).
- wp; call (butterfly64x_eq 3); wp; skip => &1 &2 |> *.
- have ->:  3 * q + q <= 32767 by rewrite /q.
+ have ->: x16_spec 20159 (C2R vx16_op).
+  by rewrite x16_spec_C2R /q /=.
+ have <-: 4*q+4*q = 8*q by ring.
+ by have <-: q+q = 2*q by ring.
+seq 6 9: (#[/:12]pre /\
+  I16u16_sb (4*q) r0{2} r0d{1} /\
+  I16u16_sb (1*q) r1{2} r1d{1} /\
+  I16u16_sb (4*q) r2{2} r2d{1} /\
+  I16u16_sb (1*q) r3{2} r3d{1} /\
+  I16u16_sb (2*q) r4{2} r4d{1} /\
+  I16u16_sb (1*q) r5{2} r5d{1} /\
+  I16u16_sb (2*q) r6{2} r6d{1} /\
+  I16u16_sb (1*q) r7{2} r7d{1} ).
+ call (invntt_butterfly64x_eq (2*q) (2*q) (1*q) (1*q) (2*q) (2*q) (1*q) (1*q)).
+ wp; ecall {2} (__shuffle1_ph (1*q) (1*q) r6b{1} r7b{1}).
+ ecall {2} (__shuffle1_ph (1*q) (1*q) r4b{1} r5b{1}).
+ ecall {2} (__shuffle1_ph (2*q) (2*q) r2b{1} r3b{1}).
+ ecall {2} (__shuffle1_ph (2*q) (2*q) r0b{1} r1b{1}).
+ ecall {2} (red16x_aux (8*q) r1b{1}).
+ ecall {2} (red16x_aux (8*q) r0b{1}).
+ have Emax: forall x, max x x = x by done. 
+ wp; skip => |> &1 &2; rewrite !Emax => |> *.
+ pose z0R := z2u256 _ _.
+ pose z1R := z2u256 _ _.
+ pose z1L := Array16.of_list _ _.
+ have ->: MAX (2 * q + 2 * q) (q + q) <= 32767 by smt().
+ have ->: qinv16u16M z0R z1R.
+  rewrite /z0R /z1R !z2u256E 1..2:// /qinv16u16M -iotaredE.
+  by rewrite /= !C2RK /zetas_inv_op !initiE //=.
+ pose xx := List.all _ _.
+ have ->: xx.
+  by rewrite /xx /z1R /z1L -iotaredE /= !z2u256E // !C2RK /zetas_inv_op /= -!inFqM_mod /q /= !Iu16_ub_of_int /q.
+ move => |> *.
+ have <-: q+q = 2*q by ring.
+ by have <-: 2*q+2*q = 4*q by ring.
+seq 6 7: (#[/:12]pre /\
+  I16u16_sb (8*q) r0{2} r0f{1} /\ (* 8 => 2 *)
+  I16u16_sb (2*q) r1{2} r1f{1} /\
+  I16u16_sb (1*q) r2{2} r2f{1} /\
+  I16u16_sb (1*q) r3{2} r3f{1} /\
+  I16u16_sb (4*q) r4{2} r4f{1} /\
+  I16u16_sb (2*q) r5{2} r5f{1} /\
+  I16u16_sb (1*q) r6{2} r6f{1} /\
+  I16u16_sb (1*q) r7{2} r7f{1} ).
+ call (invntt_butterfly64x_eq (4*q) (2*q) (1*q) (1*q) (4*q) (2*q) (1*q) (1*q)).
+ wp; ecall {2} (__shuffle2_ph (1*q) (1*q) r5d{1} r7d{1}).
+ ecall {2} (__shuffle2_ph (1*q) (1*q) r1d{1} r3d{1}).
+ ecall {2} (__shuffle2_ph (2*q) (2*q) r4d{1} r6d{1}).
+ ecall {2} (__shuffle2_ph (4*q) (4*q) r0d{1} r2d{1}).
+ have Emax: forall x, max x x = x by done. 
+ wp; skip => |> &1 &2; rewrite !Emax => |> *.
+ pose z0R := z2u256 _ _.
+ pose z1R := z2u256 _ _.
+ pose z1L := Array16.of_list _ _.
+ have ->: MAX (MAX (4*q+4*q) (2*q+2*q)) (q+q) <= 32767 by smt().
+ have ->: qinv16u16M z0R z1R.
+  rewrite /z0R /z1R !z2u256E 1..2:// /qinv16u16M -iotaredE.
+  by rewrite /= !C2RK /zetas_inv_op !initiE //=.
+ pose xx := List.all _ _.
+ have ->: xx.
+  by rewrite /xx /z0R /z1R /z1L -iotaredE /= !z2u256E // !C2RK /zetas_inv_op /= -!inFqM_mod /q /= !Iu16_ub_of_int /q.
+ move => |> *.
+ have <-: q+q = 2*q by ring.
+ have <-: 2*q+2*q = 4*q by ring.
+ by have <-: 4*q+4*q = 8*q by ring.
+seq 6 8: (#[/:12]pre /\
+  I16u16_sb (8*q) r0{2} r0h{1} /\ (* 8 => 2 *)
+  I16u16_sb (4*q) r1{2} r1h{1} /\
+  I16u16_sb (2*q) r2{2} r2h{1} /\
+  I16u16_sb (2*q) r3{2} r3h{1} /\
+  I16u16_sb (1*q) r4{2} r4h{1} /\
+  I16u16_sb (1*q) r5{2} r5h{1} /\
+  I16u16_sb (1*q) r6{2} r6h{1} /\
+  I16u16_sb (1*q) r7{2} r7h{1} ).
+ call (invntt_butterfly64x_eq (4*q) (2*q) (1*q) (1*q) (4*q) (2*q) (1*q) (1*q)).
+ wp; ecall {2} (__shuffle4_ph (1*q) (1*q) r3f{1} r7f{1}).
+ ecall {2} (__shuffle4_ph (1*q) (1*q) r2f{1} r6f{1}).
+ ecall {2} (__shuffle4_ph (2*q) (2*q) r1f{1} r5f{1}).
+ ecall {2} (__shuffle4_ph (2*q) (4*q) r0f{1} r4f{1}).
+ ecall {2} (red16x_aux (8*q) r0f{1}).
+ wp; skip => |> &1 &2; rewrite !lez_maxr 1..3:/# => |> *.
+ pose z0R := z2u256 _ _.
+ pose z1R := z2u256 _ _.
+ pose z1L := Array16.of_list _ _.
+ have ->: MAX (MAX (4*q+4*q) (2*q+2*q)) (q+q) <= 32767 by smt().
+ have ->: qinv16u16M z0R z1R.
+  rewrite /z0R /z1R !z2u256E 1..2:// /qinv16u16M -iotaredE.
+  by rewrite /= !C2RK /zetas_inv_op !initiE //=.
+ pose xx := List.all _ _.
+ have ->: xx.
+  by rewrite /xx /z0R /z1R /z1L -iotaredE /= !z2u256E // !C2RK /zetas_inv_op /= -!inFqM_mod /q /= !Iu16_ub_of_int /q.
+ move => |> *.
+ have <-: q+q = 2*q by ring.
+ have <-: 2*q+2*q = 4*q by ring.
+ by have <-: 4*q+4*q = 8*q by ring.
+seq 6 8: (#[/:12]pre /\
+  I16u16_sb (8*q) r0{2} r0j{1} /\ (* 8 => 2 *)
+  I16u16_sb (1*q) r1{2} r1j{1} /\
+  I16u16_sb (4*q) r2{2} r2j{1} /\
+  I16u16_sb (1*q) r3{2} r3j{1} /\
+  I16u16_sb (2*q) r4{2} r4j{1} /\
+  I16u16_sb (1*q) r5{2} r5j{1} /\
+  I16u16_sb (2*q) r6{2} r6j{1} /\
+  I16u16_sb (1*q) r7{2} r7j{1} ).
+ call (invntt_butterfly64x_eq (4*q) (2*q) (1*q) (1*q) (4*q) (2*q) (1*q) (1*q)).
+ wp; ecall {2} (__shuffle8_ph (1*q) (1*q) r6h{1} r7h{1}).
+ ecall {2} (__shuffle8_ph (1*q) (1*q) r4h{1} r5h{1}).
+ ecall {2} (__shuffle8_ph (2*q) (2*q) r2h{1} r3h{1}).
+ ecall {2} (__shuffle8_ph (2*q) (4*q) r0h{1} r1h{1}).
+ ecall {2} (red16x_aux (8*q) r0h{1}).
+ wp; skip => |> &1 &2; rewrite !lez_maxr 1..3:/# => |> *.
  pose z0R := VPBROADCAST_8u32 _.
  pose z1R := VPBROADCAST_8u32 _.
+ pose z1L := Array16.init _.
+ have ->: MAX (MAX (4 * q + 4 * q) (2 * q + 2 * q)) (q + q) <= 32767 by smt().
  have ->: qinv16u16M z0R z1R.
-  by rewrite /z0R /z1R /zR !z2u32E 1..2://= /VPBROADCAST_8u32 /qinv16u16M -iotaredE /R2C /zetas_op /=.
- pose z1L:= Array16.init _.
- have ->: I16u16M_ub 1 z1R z1L.
-  by rewrite /z1L /z1R /zR !z2u32E 1..2://= /VPBROADCAST_8u32 /R2C -iotaredE /= -inFqM_mod /q !Iu16_ub_of_int /#. 
- done.
-seq 6 7: (#[/:11]pre /\
-  I16u16_sb 5 r0{2} r0n{1} /\
-  I16u16_sb 5 r1{2} r1n{1} /\
-  I16u16_sb 5 r2{2} r2n{1} /\
-  I16u16_sb 5 r3{2} r3n{1} /\
-  I16u16_sb 5 r4{2} r4n{1} /\
-  I16u16_sb 5 r5{2} r5n{1} /\
-  I16u16_sb 5 r6{2} r6n{1} /\
-  I16u16_sb 5 r7{2} r7n{1} ).
- wp; call (butterfly64x_eq 4).
- ecall {2} (__shuffle8_ph 4 r3l{1} r7l{1}).
- ecall {2} (__shuffle8_ph 4 r2l{1} r6l{1}).
- ecall {2} (__shuffle8_ph 4 r1l{1} r5l{1}).
- ecall {2} (__shuffle8_ph 4 r0l{1} r4l{1}).
- wp; skip => &1 &2 |> *.
- have ->:  4 * q + q <= 32767 by rewrite /q.
- have ->: qinv16u16M (z2u256 zetas_op 204) (z2u256 zetas_op 220).
-  rewrite !z2u256E 1..2:// /qinv16u16M -iotaredE.
-  by rewrite /= !C2RK !initiE 1..32:// /zetas_op /=.
+  by rewrite /z0R /z1R /zetas_inv_op !z2u32E //= /VPBROADCAST_8u32 /qinv16u16M -iotaredE /R2C /=.
  pose xx := List.all _ _.
- have: xx.
-  by rewrite /xx -iotaredE /= !z2u256E 1..2:// !C2RK /zetas /= -!inFqM_mod /q /= !Iu16_ub_of_int /q /=.
- by rewrite /xx => {xx} -> |> *.
-seq 6 7: (#[/:11]pre /\
-  I16u16_sb 6 r0{2} r0p{1} /\
-  I16u16_sb 6 r1{2} r1p{1} /\
-  I16u16_sb 6 r2{2} r2p{1} /\
-  I16u16_sb 6 r3{2} r3p{1} /\
-  I16u16_sb 6 r4{2} r4p{1} /\
-  I16u16_sb 6 r5{2} r5p{1} /\
-  I16u16_sb 6 r6{2} r6p{1} /\
-  I16u16_sb 6 r7{2} r7p{1} ).
- wp; call (butterfly64x_eq 5).
- ecall {2} (__shuffle4_ph 5 r5n{1} r7n{1}).
- ecall {2} (__shuffle4_ph 5 r1n{1} r3n{1}).
- ecall {2} (__shuffle4_ph 5 r4n{1} r6n{1}).
- ecall {2} (__shuffle4_ph 5 r0n{1} r2n{1}).
+ have ->: xx.
+  by rewrite /xx /z1L /z1R !z2u32E //= /VPBROADCAST_8u32 /R2C -iotaredE /= -inFqM_mod /q /= /zetas_inv_op !initiE //= !Iu16_ub_of_int /q /=.
+ move => |> *.
+ have <-: q+q = 2*q by ring.
+ have <-: 2*q+2*q = 4*q by ring.
+ by have <-: 4*q+4*q = 8*q by ring.
+rcondt{2} 2; first by move=> *; inline*; auto.
+unroll{2} 11; rcondt{2} 11; first by move=> *; inline*; auto.
+seq 19 23: (#[/:2]pre /\ i{2}=1 /\ 
+   I16u16_sb (2 * q) (P2R rp{2} 0) (P2C rp8{1} 0) /\
+   I16u16_sb (4 * q) (P2R rp{2} 1) (P2C rp8{1} 1) /\
+   I16u16_sb (2 * q) (P2R rp{2} 2) (P2C rp8{1} 2) /\
+   I16u16_sb (2 * q) (P2R rp{2} 3) (P2C rp8{1} 3) /\
+   I16u16_sb (1 * q) (P2R rp{2} 4) (P2C rp8{1} 4) /\
+   I16u16_sb (1 * q) (P2R rp{2} 5) (P2C rp8{1} 5) /\
+   I16u16_sb (1 * q) (P2R rp{2} 6) (P2C rp8{1} 6) /\
+   I16u16_sb (1 * q) (P2R rp{2} 7) (P2C rp8{1} 7) /\
+   I16u16_sb (4 * q) r0{2} r0l{1} /\
+   I16u16_sb (4 * q) r1{2} r1l{1} /\
+   I16u16_sb (1 * q) r2{2} r2l{1} /\
+   I16u16_sb (1 * q) r3{2} r3l{1} /\
+   I16u16_sb (4 * q) r4{2} r4l{1} /\
+   I16u16_sb (4 * q) r5{2} r5l{1} /\
+   I16u16_sb (1 * q) r6{2} r6l{1} /\
+   I16u16_sb (1 * q) r7{2} r7l{1} ).
+ call (invntt_butterfly64x_eq (2*q) (2*q) (2*q) (2*q) (2*q) (2*q) (2*q) (2*q)).
+ wp; ecall {2} (red16x_aux (8*q) r0j{1}).
  wp; skip => &1 &2 |> *.
- have ->:  5 * q + q <= 32767 by rewrite /q.
- have ->: qinv16u16M (z2u256 zetas_op 236) (z2u256 zetas_op 252).
-  rewrite !z2u256E 1..2:// /qinv16u16M -iotaredE.
-  by rewrite /= !C2RK !initiE 1..32:// /zetas_op /=.
+ pose z0R := z2u256 _ _.
+ pose z1R := z2u256 _ _.
+ pose z2R := z2u256 _ _.
+ pose z3R := z2u256 _ _.
+ pose z1L := Array16.of_list _ _.
+ pose z3L := Array16.of_list _ _.
+ have ->: 2*q + 2*q <= 32767 by smt().
+ have ->: qinv16u16M z0R z1R.
+  rewrite /z0R /z1R !z2u256E 1..2:// /qinv16u16M -iotaredE.
+  by rewrite /= !C2RK /zetas_inv_op !initiE //=.
+ have ->: qinv16u16M z2R z3R.
+  rewrite /z2R /z3R !z2u256E 1..2:// /qinv16u16M -iotaredE.
+  by rewrite /= !C2RK /zetas_inv_op !initiE //=.
+ rewrite (P2RS rp{2}) !PUR_i //= !P2R_i //= (P2CS rp{1}) !PUC_i //= !P2C_i //= => |>. 
  pose xx := List.all _ _.
- have: xx.
-  by rewrite /xx -iotaredE /= !z2u256E 1..2:// !C2RK /zetas_op /= -!inFqM_mod /q /= !Iu16_ub_of_int /q /=.
- by rewrite /xx => {xx} -> |> *.
-seq 6 7: (#[/:11]pre /\
-  I16u16_sb 7 r0{2} r0r{1} /\
-  I16u16_sb 7 r1{2} r1r{1} /\
-  I16u16_sb 7 r2{2} r2r{1} /\
-  I16u16_sb 7 r3{2} r3r{1} /\
-  I16u16_sb 7 r4{2} r4r{1} /\
-  I16u16_sb 7 r5{2} r5r{1} /\
-  I16u16_sb 7 r6{2} r6r{1} /\
-  I16u16_sb 7 r7{2} r7r{1} ).
- wp; call (butterfly64x_eq 6).
- ecall {2} (__shuffle2_ph 6 r6p{1} r7p{1}).
- ecall {2} (__shuffle2_ph 6 r4p{1} r5p{1}).
- ecall {2} (__shuffle2_ph 6 r2p{1} r3p{1}).
- ecall {2} (__shuffle2_ph 6 r0p{1} r1p{1}).
- wp; skip => &1 &2 |> *.
- have ->:  6 * q + q <= 32767 by rewrite /q.
- have ->: qinv16u16M (z2u256 zetas_op 268) (z2u256 zetas_op 284).
-  rewrite !z2u256E 1..2:// /qinv16u16M -iotaredE.
-  by rewrite /= !C2RK !initiE 1..32:// /zetas_op /=.
+ have ->: xx.
+  by rewrite /xx /z1R /z1L -iotaredE /= !z2u256E // !C2RK /zetas_inv_op /= -!inFqM_mod /q /= !Iu16_ub_of_int /q.
+ clear xx; pose xx := List.all _ _.
+ have ->: xx.
+  by rewrite /xx /z3R /z3L -iotaredE /= !z2u256E // !C2RK /zetas_inv_op /= -!inFqM_mod /q /= !Iu16_ub_of_int /q.
+ move => |> *.
+ by have <-: 2*q+2*q = 4*q by ring.
+seq 2 4: (#[/:11]pre /\ x16_spec 20159 vx16{2} /\
+   I16u16_sb (8 * q) r0{2} r0m{1} /\ (* 8 ==> 2 *)
+   I16u16_sb (8 * q) r1{2} r1m{1} /\ (* 8 ==> 2 *)
+   I16u16_sb (2 * q) r2{2} r2m{1} /\
+   I16u16_sb (2 * q) r3{2} r3m{1} /\
+   I16u16_sb (1 * q) r4{2} r4m{1} /\
+   I16u16_sb (1 * q) r5{2} r5m{1} /\
+   I16u16_sb (1 * q) r6{2} r6m{1} /\
+   I16u16_sb (1 * q) r7{2} r7m{1} ).
+ call (invntt_butterfly64x_eq (4*q) (4*q) (1*q) (1*q) (4*q) (4*q) (1*q) (1*q)).
+ wp; skip => |> &1 &2 *.
+ pose z0R := z2u256 _ _.
+ pose z1R := z2u256 _ _.
+ pose z1L := Array16.of_list _ _.
+ have ->: MAX (4 * q + 4 * q) (q + q) <= 32767 by smt().
+ have ->: qinv16u16M z0R z1R.
+  rewrite /z0R /z1R !z2u256E 1..2:// /qinv16u16M -iotaredE.
+  by rewrite /= !C2RK /zetas_inv_op !initiE //=.
  pose xx := List.all _ _.
- have: xx.
-  by rewrite /xx -iotaredE /= !z2u256E 1..2:// !C2RK /zetas_op /= -!inFqM_mod /q /= !Iu16_ub_of_int /q.
- by rewrite /xx => {xx} -> |> *.
-seq 6 7: (#[/:11]pre /\
-  I16u16_sb 8 r0{2} r0t{1} /\
-  I16u16_sb 8 r1{2} r1t{1} /\
-  I16u16_sb 8 r2{2} r2t{1} /\
-  I16u16_sb 8 r3{2} r3t{1} /\
-  I16u16_sb 8 r4{2} r4t{1} /\
-  I16u16_sb 8 r5{2} r5t{1} /\
-  I16u16_sb 8 r6{2} r6t{1} /\
-  I16u16_sb 8 r7{2} r7t{1} ).
- wp; call (butterfly64x_eq 7).
- ecall {2} (__shuffle1_ph 7 r3r{1} r7r{1}).
- ecall {2} (__shuffle1_ph 7 r2r{1} r6r{1}).
- ecall {2} (__shuffle1_ph 7 r1r{1} r5r{1}).
- ecall {2} (__shuffle1_ph 7 r0r{1} r4r{1}).
- wp; skip => &1 &2 |> *.
- have ->:  7 * q + q <= 32767 by rewrite /q.
- have ->: qinv16u16M (z2u256 zetas_op 300) (z2u256 zetas_op 316).
-  rewrite !z2u256E 1..2:// /qinv16u16M -iotaredE.
-  by rewrite /= !C2RK !initiE 1..32:// /zetas_op /=.
+ have ->: xx.
+  by rewrite /xx /z1R /z1L -iotaredE /= !z2u256E // !C2RK /zetas_inv_op /= -!inFqM_mod /q /= !Iu16_ub_of_int /q.
+ move => |> *.
+ have ->: x16_spec 20159 (C2R vx16_op).
+  by rewrite x16_spec_C2R /q /=.
+ have <-: 4*q+4*q = 8*q by ring.
+ by have <-: q+q = 2*q by ring.
+seq 6 9: (#[/:12]pre /\
+   I16u16_sb (4*q) r0{2} r0o{1} /\
+   I16u16_sb (1*q) r1{2} r1o{1} /\
+   I16u16_sb (4*q) r2{2} r2o{1} /\
+   I16u16_sb (1*q) r3{2} r3o{1} /\
+   I16u16_sb (2*q) r4{2} r4o{1} /\
+   I16u16_sb (1*q) r5{2} r5o{1} /\
+   I16u16_sb (2*q) r6{2} r6o{1} /\
+   I16u16_sb (1*q) r7{2} r7o{1} ).
+ call (invntt_butterfly64x_eq (2*q) (2*q) (1*q) (1*q) (2*q) (2*q) (1*q) (1*q)).
+ wp; ecall {2} (__shuffle1_ph (1*q) (1*q) r6m{1} r7m{1}).
+ ecall {2} (__shuffle1_ph (1*q) (1*q) r4m{1} r5m{1}).
+ ecall {2} (__shuffle1_ph (2*q) (2*q) r2m{1} r3m{1}).
+ ecall {2} (__shuffle1_ph (2*q) (2*q) r0m{1} r1m{1}).
+ ecall {2} (red16x_aux (8*q) r1m{1}).
+ ecall {2} (red16x_aux (8*q) r0m{1}).
+ have Emax: forall x, max x x = x by done. 
+ wp; skip => |> &1 &2; rewrite !Emax => |> *.
+ pose z0R := z2u256 _ _.
+ pose z1R := z2u256 _ _.
+ pose z1L := Array16.of_list _ _.
+ have ->: MAX (2 * q + 2 * q) (q + q) <= 32767 by smt().
+ have ->: qinv16u16M z0R z1R.
+  rewrite /z0R /z1R !z2u256E 1..2:// /qinv16u16M -iotaredE.
+  by rewrite /= !C2RK /zetas_inv_op !initiE //=.
  pose xx := List.all _ _.
- have: xx.
-  by rewrite /xx -iotaredE /= !z2u256E 1..2:// !C2RK /zetas_op /= -!inFqM_mod /q /= !Iu16_ub_of_int /q /=.
- by rewrite /xx => {xx} -> |> *.
-wp; ecall {2} (__red16x_ph r7u{1}).
-ecall {2} (__red16x_ph r3u{1}).
-ecall {2} (__red16x_ph r5u{1}).
-ecall {2} (__red16x_ph r1u{1}).
-ecall {2} (__red16x_ph r6u{1}).
-ecall {2} (__red16x_ph r2u{1}).
-ecall {2} (__red16x_ph r4u{1}).
-ecall {2} (__red16x_ph r0u{1}).
-wp; call (butterfly64x_eq 8).
-wp; skip => &1 &2 |> *.
-have ->:  8 * q + q <= 32767 by rewrite /q.
-have ->: qinv16u16M (z2u256 zetas_op 332) (z2u256 zetas_op 348).
- rewrite !z2u256E 1..2:// /qinv16u16M -iotaredE.
- by rewrite /= !C2RK !initiE 1..32:// /zetas_op /=.
-have ->: qinv16u16M (z2u256 zetas_op 364) (z2u256 zetas_op 380).
- rewrite !z2u256E 1..2:// /qinv16u16M -iotaredE.
- by rewrite /= !C2RK !initiE 1..32:// /zetas_op /=.
+ have ->: xx.
+  by rewrite /xx /z1R /z1L -iotaredE /= !z2u256E // !C2RK /zetas_inv_op /= -!inFqM_mod /q /= !Iu16_ub_of_int /q.
+ move => |> *.
+ have <-: q+q = 2*q by ring.
+ by have <-: 2*q+2*q = 4*q by ring.
+seq 6 7: (#[/:12]pre /\
+   I16u16_sb (8*q) r0{2} r0q{1} /\ (* 8 => 2 *)
+   I16u16_sb (2*q) r1{2} r1q{1} /\
+   I16u16_sb (1*q) r2{2} r2q{1} /\
+   I16u16_sb (1*q) r3{2} r3q{1} /\
+   I16u16_sb (4*q) r4{2} r4q{1} /\
+   I16u16_sb (2*q) r5{2} r5q{1} /\
+   I16u16_sb (1*q) r6{2} r6q{1} /\
+   I16u16_sb (1*q) r7{2} r7q{1} ).
+ call (invntt_butterfly64x_eq (4*q) (2*q) (1*q) (1*q) (4*q) (2*q) (1*q) (1*q)).
+ wp; ecall {2} (__shuffle2_ph (1*q) (1*q) r5o{1} r7o{1}).
+ ecall {2} (__shuffle2_ph (1*q) (1*q) r1o{1} r3o{1}).
+ ecall {2} (__shuffle2_ph (2*q) (2*q) r4o{1} r6o{1}).
+ ecall {2} (__shuffle2_ph (4*q) (4*q) r0o{1} r2o{1}).
+ have Emax: forall x, max x x = x by done.
+ wp; skip => |> &1 &2; rewrite !Emax => |> *.
+ pose z0R := z2u256 _ _.
+ pose z1R := z2u256 _ _.
+ pose z1L := Array16.of_list _ _.
+ have ->: MAX (MAX (4*q+4*q) (2*q+2*q)) (q+q) <= 32767 by smt().
+ have ->: qinv16u16M z0R z1R.
+  rewrite /z0R /z1R !z2u256E 1..2:// /qinv16u16M -iotaredE.
+  by rewrite /= !C2RK /zetas_inv_op !initiE //=.
+ pose xx := List.all _ _.
+ have ->: xx.
+  by rewrite /xx /z1R /z1L -iotaredE /= !z2u256E // !C2RK /zetas_inv_op /= -!inFqM_mod /q /= !Iu16_ub_of_int /q.
+ move => |> *.
+ have <-: q+q = 2*q by ring.
+ have <-: 2*q+2*q = 4*q by ring.
+ by have <-: 4*q+4*q = 8*q by ring.
+seq 6 8: (#[/:12]pre /\
+  I16u16_sb (8*q) r0{2} r0s{1} /\ (* 8 => 2 *)
+  I16u16_sb (4*q) r1{2} r1s{1} /\
+  I16u16_sb (2*q) r2{2} r2s{1} /\
+  I16u16_sb (2*q) r3{2} r3s{1} /\
+  I16u16_sb (1*q) r4{2} r4s{1} /\
+  I16u16_sb (1*q) r5{2} r5s{1} /\
+  I16u16_sb (1*q) r6{2} r6s{1} /\
+  I16u16_sb (1*q) r7{2} r7s{1} ).
+ call (invntt_butterfly64x_eq (4*q) (2*q) (1*q) (1*q) (4*q) (2*q) (1*q) (1*q)).
+ wp; ecall {2} (__shuffle4_ph (1*q) (1*q) r3q{1} r7q{1}).
+ ecall {2} (__shuffle4_ph (1*q) (1*q) r2q{1} r6q{1}).
+ ecall {2} (__shuffle4_ph (2*q) (2*q) r1q{1} r5q{1}).
+ ecall {2} (__shuffle4_ph (2*q) (4*q) r0q{1} r4q{1}).
+ ecall {2} (red16x_aux (8*q) r0q{1}).
+ wp; skip => |> &1 &2; rewrite !lez_maxr 1..3:/# => |> *.
+ pose z0R := z2u256 _ _.
+ pose z1R := z2u256 _ _.
+ pose z1L := Array16.of_list _ _.
+ have ->: MAX (MAX (4*q+4*q) (2*q+2*q)) (q+q) <= 32767 by smt().
+ have ->: qinv16u16M z0R z1R.
+  rewrite /z0R /z1R !z2u256E 1..2:// /qinv16u16M -iotaredE.
+  by rewrite /= !C2RK /zetas_inv_op !initiE //=.
+ pose xx := List.all _ _.
+ have ->: xx.
+  by rewrite /xx /z0R /z1R /z1L -iotaredE /= !z2u256E // !C2RK /zetas_inv_op /= -!inFqM_mod /q /= !Iu16_ub_of_int /q.
+ move => |> *.
+ have <-: q+q = 2*q by ring.
+ have <-: 2*q+2*q = 4*q by ring.
+ by have <-: 4*q+4*q = 8*q by ring.
+seq 6 8: (#[/:12]pre /\
+  I16u16_sb (8*q) r0{2} r0u{1} /\ (* 8 => 2 *)
+  I16u16_sb (1*q) r1{2} r1u{1} /\
+  I16u16_sb (4*q) r2{2} r2u{1} /\
+  I16u16_sb (1*q) r3{2} r3u{1} /\
+  I16u16_sb (2*q) r4{2} r4u{1} /\
+  I16u16_sb (1*q) r5{2} r5u{1} /\
+  I16u16_sb (2*q) r6{2} r6u{1} /\
+  I16u16_sb (1*q) r7{2} r7u{1} ).
+ call (invntt_butterfly64x_eq (4*q) (2*q) (1*q) (1*q) (4*q) (2*q) (1*q) (1*q)).
+ wp; ecall {2} (__shuffle8_ph (1*q) (1*q) r6s{1} r7s{1}).
+ ecall {2} (__shuffle8_ph (1*q) (1*q) r4s{1} r5s{1}).
+ ecall {2} (__shuffle8_ph (2*q) (2*q) r2s{1} r3s{1}).
+ ecall {2} (__shuffle8_ph (2*q) (4*q) r0s{1} r1s{1}).
+ ecall {2} (red16x_aux (8*q) r0s{1}).
+ wp; skip => |> &1 &2; rewrite !lez_maxr 1..3:/# => |> *.
+ pose z0R := VPBROADCAST_8u32 _.
+ pose z1R := VPBROADCAST_8u32 _.
+ pose z1L := Array16.init _.
+ have ->: MAX (MAX (4 * q + 4 * q) (2 * q + 2 * q)) (q + q) <= 32767 by smt().
+ have ->: qinv16u16M z0R z1R.
+  by rewrite /z0R /z1R /zetas_inv_op !z2u32E //= /VPBROADCAST_8u32 /qinv16u16M -iotaredE /R2C /=.
+ pose xx := List.all _ _.
+ have ->: xx.
+  by rewrite /xx /z1L /z1R !z2u32E //= /VPBROADCAST_8u32 /R2C -iotaredE /= -inFqM_mod /q /= /zetas_inv_op !initiE //= !Iu16_ub_of_int /q /=.
+ move => |> *.
+ have <-: q+q = 2*q by ring.
+ have <-: 2*q+2*q = 4*q by ring.
+ by have <-: 4*q+4*q = 8*q by ring.
+rcondf{2} 2; first by move=> *; inline*; auto.
+rcondf{2} 7; first by move=> *; inline*; auto.
+unroll{2} 12; rcondt{2} 12; first by move => *; inline*; auto.
+rcondt{2} 12; first by move => *; inline*; auto.
+seq 13 33: (#[/:2]pre /\ x16_spec (-10079) flox16{2} /\
+            x16_spec 1441 fhix16{2} /\ i{2}=1 /\ 
+   I16u16_sb (1 * q) (P2R rp{2} 0) (mul16x1 r0a{1} (inFq 3303)) /\
+   I16u16_sb (1 * q) (P2R rp{2} 1) (mul16x1 r1a{1} (inFq 3303)) /\
+   I16u16_sb (1 * q) (P2R rp{2} 2) (mul16x1 r2a{1} (inFq 3303)) /\
+   I16u16_sb (1 * q) (P2R rp{2} 3) (mul16x1 r3a{1} (inFq 3303)) /\
+   I16u16_sb (1 * q) (P2R rp{2} 4) r0b{1} /\
+   I16u16_sb (1 * q) (P2R rp{2} 5) r1b{1} /\
+   I16u16_sb (1 * q) (P2R rp{2} 6) r2b{1} /\
+   I16u16_sb (1 * q) (P2R rp{2} 7) r3b{1} /\
+   I16u16_sb (1 * q) (P2R rp{2} 8) (mul16x1 r4a{1} (inFq 3303)) /\
+   I16u16_sb (1 * q) (P2R rp{2} 9) (mul16x1 r5a{1} (inFq 3303)) /\
+   I16u16_sb (1 * q) (P2R rp{2} 10) (mul16x1 r6a{1} (inFq 3303)) /\
+   I16u16_sb (1 * q) (P2R rp{2} 11) (mul16x1 r7a{1} (inFq 3303)) /\
+   I16u16_sb (1 * q) (P2R rp{2} 12) r4b{1} /\
+   I16u16_sb (1 * q) (P2R rp{2} 13) r5b{1} /\
+   I16u16_sb (1 * q) (P2R rp{2} 14) r6b{1} /\
+   I16u16_sb (1 * q) (P2R rp{2} 15) r7b{1} /\
+   zeta0{2} = VPBROADCAST_8u32 (z2u32 zetas_inv_op 392) /\
+   zeta1{2} = VPBROADCAST_8u32 (z2u32 zetas_inv_op 394) /\
+   fhix16{2} = C2R fhix16_op /\
+   flox16{2} = C2R flox16_op /\
+   zeta0{1} = Array16.init (fun (_ : int) => inFq 1600) ).
+ wp.
+ ecall {2} (fq_mulprecomp16x_aux (4*q) r3a{1}).
+ ecall {2} (fq_mulprecomp16x_aux (4*q) r2a{1}).
+ ecall {2} (fq_mulprecomp16x_aux (8*q) r1a{1}).
+ ecall {2} (fq_mulprecomp16x_aux (4*q) r0a{1}).
+ wp; call (invntt_butterfly64x_eq_last (inFq 3303) (2*q) (4*q) (2*q) (2*q) (2*q) (4*q) (2*q) (2*q)).
+ wp; ecall {2} (red16x_aux (8*q) r0u{1}).
+ skip => |> &1 &2 *. (* rewrite !lez_maxl 1..3:/# => |> *.*)
+ pose z0R := VPBROADCAST_8u32 _.
+ pose z1R := VPBROADCAST_8u32 _.
+ pose z1L := Array16.init _.
+ have ->: MAX (MAX (2*q+2*q) (4*q+4*q)) (2*q+2*q) <= 32767 by smt().
+ rewrite (P2RS rp{2}) !PUR_i //= !P2R_i //= (P2CS rp8{1}) !PUC_i //= !P2C_i //= => |>.
+ have ->: qinv16u16M z0R z1R.
+  by rewrite /z0R /z1R /zetas_inv_op !z2u32E //= /VPBROADCAST_8u32 /qinv16u16M -iotaredE /R2C /=.
+ pose xx := List.all _ _.
+ have ->: xx.
+  by rewrite /xx /z1L /z1R !z2u32E //= /VPBROADCAST_8u32 /R2C -iotaredE /= -!inFqM_mod !inFqK /q /= /zetas_inv_op !initiE //= !Iu16_ub_of_int /q /=.
+ move => |> *.
+ have ->: x16_spec 1441 (C2R fhix16_op).
+  by rewrite x16_spec_C2R /=.
+ have ->: x16_spec (-10079) (C2R flox16_op).
+  by rewrite x16_spec_C2R /=.
+ have ->: qinv16u16M (C2R flox16_op) (C2R fhix16_op).
+  by rewrite /flox16_op /fhix16_op /qinv16u16M !C2RK //= -iotaredE /=. 
+ have <-: 2 * q + 2 * q = 4 * q by ring.
+ have <-: 4 * q + 4 * q = 8 * q by ring.
+ move => |> *.
+ by rewrite !PUR_i //= !P2R_i //=.
+unroll{2} 1; rcondt{2} 1; first by auto.
+rcondf{2} 1; first by auto.
+rcondf{2} 23; first by move=> *; inline*; auto.
+wp.
+ecall {2} (fq_mulprecomp16x_aux (2*q) r3c{1}).
+ecall {2} (fq_mulprecomp16x_aux (2*q) r2c{1}).
+ecall {2} (fq_mulprecomp16x_aux (2*q) r1c{1}).
+ecall {2} (fq_mulprecomp16x_aux (2*q) r0c{1}).
+wp; call (invntt_butterfly64x_eq_last (inFq 3303) (1*q) (1*q) (1*q) (1*q) (1*q) (1*q) (1*q) (1*q)).
+wp; skip => |> &1 &2 *.
+pose z0R := VPBROADCAST_8u32 _.
+pose z1R := VPBROADCAST_8u32 _.
+pose z1L := Array16.init _.
+have ->: q+q <= 32767 by smt().
+have ->: qinv16u16M z0R z1R.
+ by rewrite /z0R /z1R /zetas_inv_op !z2u32E //= /VPBROADCAST_8u32 /qinv16u16M -iotaredE /R2C /=.
 pose xx := List.all _ _.
-have: xx.
- by rewrite /xx -iotaredE /= !z2u256E 1..2:// !C2RK /zetas_op /= -!inFqM_mod /q /= !Iu16_ub_of_int /q /=.
-rewrite /xx => {xx} ->; pose xx := List.all _ _.
-have: xx.
- by rewrite /xx -iotaredE /= !z2u256E 1..2:// !C2RK /zetas_op /= -!inFqM_mod /q /= !Iu16_ub_of_int /q /=.
-rewrite /xx => {xx} -> |> *.
-have Hvx16: x16_spec 20159 (C2R vx16_op).
- by rewrite x16_spec_C2R /q /=.
+have ->: xx.
+ by rewrite /xx /z1L /z1R !z2u32E //= /VPBROADCAST_8u32 /R2C -iotaredE /= -!inFqM_mod !inFqK /q /= /zetas_inv_op !initiE //= !Iu16_ub_of_int /q /=.
 move => |> *.
-by rewrite (P2RS rp{2}) (P2CS rp8{1}) /= !PUR_i //= !PUC_i //= -{2}iotaredE /= !P2R_i //= !P2C_i //=.
+have ->: qinv16u16M (C2R flox16_op) (C2R fhix16_op).
+ by rewrite /flox16_op /fhix16_op /qinv16u16M !C2RK //= -iotaredE /=. 
+move => |> *.
+have <-: q + q = 2 * q by ring.
+move => |> *.
+rewrite (P2RS rp{2}) !PUR_i //=.
+rewrite -{2}iotaredE /=. 
+by rewrite !P2R_i //= !P2C_mul16x1 //=.
 qed.
 
-admit.
-qed.
-
-equiv __invntt_level6_eq:
- NTT_AVX.__invntt_level6 ~ Jkem_avx2.M.__invntt_level6:
- I256u16_sb 2 rp{2} rp{1} ==> I256u16_sb 3 res{2} res{1}.
-proof.
-admitted.
-
-
-equiv _poly_invntt_eq:
- NTT_AVX.invntt ~Jkem_avx2.M._poly_invntt:
- r{1}=lift_array256 rp{2} /\ signed_bound_cxq rp{2} 0 256 2 ==>
- res{1}=lift_array256 res{2} /\
- signed_bound_cxq rp{2} 0 256 1. (* pos_bound256_cxq res{2} 0 256 2.*)
-proof.
-proc.
-conseq (_: I256u16_sb 2 rp{2} r{1} ==> I256u16_ub 2 rp{2} rp2{1} ).
-  by move=> &1 &2; rewrite I256u16_sbE.
- by move => &1 &2 /= ???; rewrite -I256u16_ubE.
-call __invntt_level6_eq.
-by call __invntt_level0t5_eq.
-qed.
-
-
-*)
